<?xml version="1.0"?>
<rdf:RDF xmlns="https://w3id.org/transmodel/facilities#"
     xml:base="https://w3id.org/transmodel/facilities"
     xmlns:cc="http://creativecommons.org/ns#"
     xmlns:dc="http://purl.org/dc/elements/1.1/"
     xmlns:owl="http://www.w3.org/2002/07/owl#"
     xmlns:rdf="http://www.w3.org/1999/02/22-rdf-syntax-ns#"
     xmlns:xml="http://www.w3.org/XML/1998/namespace"
     xmlns:xsd="http://www.w3.org/2001/XMLSchema#"
     xmlns:rdfs="http://www.w3.org/2000/01/rdf-schema#"
     xmlns:vann="http://purl.org/vocab/vann/"
     xmlns:tmfac="https://w3id.org/transmodel/facilities#"
     xmlns:tmkos="https://w3id.org/transmodel/kos/"
     xmlns:tmorg="https://w3id.org/transmodel/organisations#"
     xmlns:tmfare="https://w3id.org/transmodel/fares#"
     xmlns:tmcommons="https://w3id.org/transmodel/commons#"
     xmlns:tmjourney="https://w3id.org/transmodel/journeys#"
     xmlns:tmkosfare="https://w3id.org/transmodel/kos/fares/"
     xmlns:tmkoscommons="https://w3id.org/transmodel/kos/commons/"
     xmlns:tmkosjourney="https://w3id.org/transmodel/kos/journeys/"
     xmlns:tmkosfacility="https://w3id.org/transmodel/kos/facilities/"
     xmlns:tmkosorg="https://w3id.org/transmodel/kos/organisations/">
    <owl:Ontology rdf:about="https://w3id.org/transmodel/facilities#">
        <owl:versionIRI rdf:resource="https://w3id.org/transmodel/facilities/0.2"/>
        <cc:license rdf:resource="http://creativecommons.org/licenses/by/4.0/"/>
        <dc:creator>Adolfo Antón Bravo (Ontology Engineering Group - Universidad Politécnica de Madrid)</dc:creator>
        <dc:creator>Oscar Corcho (Ontology Engineering Group - Universidad Politécnica de Madrid)</dc:creator>
        <dc:date>2019-10-06</dc:date>
        <dc:description xml:lang="en">Module of the Transmodel Ontology focused on facilities. This ontology provides support to the NeTEx model. Visit https://github.com/oeg-upm/transmodel-ontology</dc:description>
        <dc:identifier>https://w3id.org/transmodel/facilities</dc:identifier>
        <dc:rights>Creative Commons Attribution 4.0 International (CC BY 4.0)</dc:rights>
        <dc:title xml:lang="en">Transmodel Ontology - Facilities</dc:title>
        <vann:preferredNamespaceUri rdf:resource="https://w3id.org/transmodel/facilities#"/>
        <rdfs:comment xml:lang="en">Module of the Transmodel Ontology focused on facilities. This ontology provides support to the NeTEx model. Visit https://github.com/oeg-upm/transmodel-ontology</rdfs:comment>
        <rdfs:label xml:lang="en">Transmodel Ontology - Facilities</rdfs:label>
        <rdfs:seeAlso xml:lang="en">https://github.com/oeg-upm/transmodel-ontology</rdfs:seeAlso>
        <owl:versionInfo xml:lang="en">This is the initial version of the module on Facilities, after considering the UML models and XSD descriptions of Transmodel and NeTEx</owl:versionInfo>
    </owl:Ontology>
    


    <!-- 
    ///////////////////////////////////////////////////////////////////////////////////////
    //
    // Annotation properties
    //
    ///////////////////////////////////////////////////////////////////////////////////////
     -->

    


    <!-- http://creativecommons.org/ns#license -->

    <owl:AnnotationProperty rdf:about="http://creativecommons.org/ns#license"/>
    


    <!-- http://purl.org/dc/elements/1.1/creator -->

    <owl:AnnotationProperty rdf:about="http://purl.org/dc/elements/1.1/creator"/>
    


    <!-- http://purl.org/dc/elements/1.1/date -->

    <owl:AnnotationProperty rdf:about="http://purl.org/dc/elements/1.1/date"/>
    


    <!-- http://purl.org/dc/elements/1.1/description -->

    <owl:AnnotationProperty rdf:about="http://purl.org/dc/elements/1.1/description"/>
    


    <!-- http://purl.org/dc/elements/1.1/identifier -->

    <owl:AnnotationProperty rdf:about="http://purl.org/dc/elements/1.1/identifier"/>
    


    <!-- http://purl.org/dc/elements/1.1/rights -->

    <owl:AnnotationProperty rdf:about="http://purl.org/dc/elements/1.1/rights"/>
    


    <!-- http://purl.org/dc/elements/1.1/title -->

    <owl:AnnotationProperty rdf:about="http://purl.org/dc/elements/1.1/title"/>
    


    <!-- http://purl.org/vocab/vann/preferredNamespaceUri -->

    <owl:AnnotationProperty rdf:about="http://purl.org/vocab/vann/preferredNamespaceUri"/>
    


    <!-- https://w3id.org/transmodel/facilities#author -->

    <owl:AnnotationProperty rdf:about="https://w3id.org/transmodel/facilities#author"/>
    


    <!-- https://w3id.org/transmodel/facilities#creator -->

    <owl:AnnotationProperty rdf:about="https://w3id.org/transmodel/facilities#creator"/>
    


    <!-- https://w3id.org/transmodel/facilities#description -->

    <owl:AnnotationProperty rdf:about="https://w3id.org/transmodel/facilities#description">
        <rdfs:range rdf:resource="http://www.w3.org/2000/01/rdf-schema#Literal"/>
        <rdfs:domain rdf:resource="https://w3id.org/transmodel/facilities#MeetingPointService"/>
    </owl:AnnotationProperty>
    


    <!-- https://w3id.org/transmodel/facilities#mbox -->

    <owl:AnnotationProperty rdf:about="https://w3id.org/transmodel/facilities#mbox"/>
    


    <!-- https://w3id.org/transmodel/facilities#name -->

    <owl:AnnotationProperty rdf:about="https://w3id.org/transmodel/facilities#name">
        <rdfs:range rdf:resource="http://www.w3.org/2000/01/rdf-schema#Literal"/>
    </owl:AnnotationProperty>
    


    <!-- 
    ///////////////////////////////////////////////////////////////////////////////////////
    //
    // Datatypes
    //
    ///////////////////////////////////////////////////////////////////////////////////////
     -->

    


    <!-- http://www.w3.org/2001/XMLSchema#duration -->

    <rdfs:Datatype rdf:about="http://www.w3.org/2001/XMLSchema#duration"/>
    


    <!-- http://www.w3.org/2001/XMLSchema#string -->

    <rdf:Description rdf:about="http://www.w3.org/2001/XMLSchema#string">
        <owl:equivalentClass rdf:resource="http://www.w3.org/2001/XMLSchema#duration"/>
    </rdf:Description>
    


    <!-- 
    ///////////////////////////////////////////////////////////////////////////////////////
    //
    // Object Properties
    //
    ///////////////////////////////////////////////////////////////////////////////////////
     -->

    


    <!-- http://www.w3.org/2004/02/skos/core#inScheme -->

    <owl:ObjectProperty rdf:about="http://www.w3.org/2004/02/skos/core#inScheme"/>
    


    <!-- https://w3id.org/transmodel/commons#in -->

    <owl:ObjectProperty rdf:about="https://w3id.org/transmodel/commons#in"/>
    


    <!-- https://w3id.org/transmodel/facilities#OBJECTPROPERTIESTOREVIEW -->

    <owl:ObjectProperty rdf:about="https://w3id.org/transmodel/facilities#OBJECTPROPERTIESTOREVIEW"/>
    


    <!-- https://w3id.org/transmodel/facilities#accessedBy -->

    <owl:ObjectProperty rdf:about="https://w3id.org/transmodel/facilities#accessedBy">
        <rdfs:comment xml:lang="en">This property sets the relationship between Site and Entrance</rdfs:comment>
        <rdfs:label xml:lang="en">accessed By</rdfs:label>
    </owl:ObjectProperty>
    


    <!-- https://w3id.org/transmodel/facilities#accessibilityAssessment -->

    <owl:ObjectProperty rdf:about="https://w3id.org/transmodel/facilities#accessibilityAssessment">
        <rdfs:subPropertyOf rdf:resource="http://www.w3.org/2002/07/owl#topObjectProperty"/>
        <rdfs:range rdf:resource="https://w3id.org/transmodel/facilities#AccessibilityAssessment"/>
        <rdfs:comment xml:lang="en">TODO: Determine whether this should be moved to another module if the concept AccessibilityAssessment is moved as well</rdfs:comment>
        <rdfs:comment xml:lang="en">This property is used to relate a site element, a facility, etc., with a specific accessibility assessment. In some of the UML models of Transmodel this property is name as characerisedBy</rdfs:comment>
        <rdfs:label xml:lang="en">accessibility Assessment</rdfs:label>
    </owl:ObjectProperty>
    


    <!-- https://w3id.org/transmodel/facilities#accessibilityLimitation -->

    <owl:ObjectProperty rdf:about="https://w3id.org/transmodel/facilities#accessibilityLimitation">
        <rdfs:subPropertyOf rdf:resource="https://w3id.org/transmodel/facilities#OBJECTPROPERTIESTOREVIEW"/>
        <rdfs:domain rdf:resource="https://w3id.org/transmodel/facilities#Facility"/>
        <rdfs:label xml:lang="en">accessibilityLimitation</rdfs:label>
    </owl:ObjectProperty>
    


    <!-- https://w3id.org/transmodel/facilities#accommodationFacility -->

    <owl:ObjectProperty rdf:about="https://w3id.org/transmodel/facilities#accommodationFacility">
        <rdfs:subPropertyOf rdf:resource="https://w3id.org/transmodel/facilities#facilityType"/>
        <rdfs:domain rdf:resource="https://w3id.org/transmodel/facilities#Accommodation"/>
        <rdfs:range>
            <owl:Class>
                <owl:intersectionOf rdf:parseType="Collection">
                    <rdf:Description rdf:about="http://www.w3.org/2004/02/skos/core#Concept"/>
                    <owl:Restriction>
                        <owl:onProperty rdf:resource="http://www.w3.org/2004/02/skos/core#inScheme"/>
                        <owl:hasValue rdf:resource="https://w3id.org/transmodel/kos/facilities/FacilityType"/>
                    </owl:Restriction>
                </owl:intersectionOf>
            </owl:Class>
        </rdfs:range>
        <rdfs:comment xml:lang="en">TODO: the range of this property may be further restricted to those SKOS concepts that also comply with skos:broader tmkosfacility:FacilityType/AccomodationFacilityType</rdfs:comment>
        <rdfs:comment xml:lang="en">This property restricts the type of facility to one specific for accommodation from the SKOS codelist for types of facilities, including, for example, values like seating, sleeper, couchette, special seating, reclining seats, standing, etc.</rdfs:comment>
        <rdfs:label xml:lang="en">accommodation facility</rdfs:label>
    </owl:ObjectProperty>
    


    <!-- https://w3id.org/transmodel/facilities#accomodation -->

    <owl:ObjectProperty rdf:about="https://w3id.org/transmodel/facilities#accomodation">
        <rdfs:subPropertyOf rdf:resource="https://w3id.org/transmodel/facilities#OBJECTPROPERTIESTOREVIEW"/>
        <rdfs:domain rdf:resource="https://w3id.org/transmodel/journeys#Service"/>
        <rdfs:label xml:lang="en">accomodation</rdfs:label>
    </owl:ObjectProperty>
    


    <!-- https://w3id.org/transmodel/facilities#activateEquipment -->

    <owl:ObjectProperty rdf:about="https://w3id.org/transmodel/facilities#activateEquipment">
        <rdfs:subPropertyOf rdf:resource="https://w3id.org/transmodel/facilities#OBJECTPROPERTIESTOREVIEW"/>
        <rdfs:domain rdf:resource="https://w3id.org/transmodel/facilities#Passenger"/>
        <rdfs:range rdf:resource="https://w3id.org/transmodel/facilities#Equipment"/>
        <rdfs:label xml:lang="en">activateEquipment</rdfs:label>
    </owl:ObjectProperty>
    


    <!-- https://w3id.org/transmodel/facilities#activationAssignment -->

    <owl:ObjectProperty rdf:about="https://w3id.org/transmodel/facilities#activationAssignment">
        <rdfs:subPropertyOf rdf:resource="https://w3id.org/transmodel/facilities#OBJECTPROPERTIESTOREVIEW"/>
        <rdfs:label xml:lang="en">activationAssignment</rdfs:label>
    </owl:ObjectProperty>
    


    <!-- https://w3id.org/transmodel/facilities#availableAt -->

    <owl:ObjectProperty rdf:about="https://w3id.org/transmodel/facilities#availableAt">
        <rdfs:domain rdf:resource="https://w3id.org/transmodel/facilities#SiteFacilitySet"/>
        <rdfs:range rdf:resource="https://w3id.org/transmodel/facilities#Site"/>
        <rdfs:comment xml:lang="en">TODO: Check whether this property is also applicable to other things beyond Site Facility Sets</rdfs:comment>
        <rdfs:comment xml:lang="en">This property relates a Site Facility Set with a Site</rdfs:comment>
        <rdfs:label xml:lang="en">available At</rdfs:label>
    </owl:ObjectProperty>
    


    <!-- https://w3id.org/transmodel/facilities#boardingPermission -->

    <owl:ObjectProperty rdf:about="https://w3id.org/transmodel/facilities#boardingPermission">
        <rdfs:subPropertyOf rdf:resource="https://w3id.org/transmodel/facilities#facilityType"/>
        <rdfs:domain rdf:resource="https://w3id.org/transmodel/facilities#OnboardStay"/>
        <rdfs:range>
            <owl:Class>
                <owl:intersectionOf rdf:parseType="Collection">
                    <rdf:Description rdf:about="http://www.w3.org/2004/02/skos/core#Concept"/>
                    <owl:Restriction>
                        <owl:onProperty rdf:resource="http://www.w3.org/2004/02/skos/core#inScheme"/>
                        <owl:hasValue rdf:resource="https://w3id.org/transmodel/kos/facilities/FacilityType"/>
                    </owl:Restriction>
                </owl:intersectionOf>
            </owl:Class>
        </rdfs:range>
        <rdfs:comment xml:lang="en">TODO: the range of this property may be further restricted to those SKOS concepts that also comply with skos:broader tmkosfacility:FacilityType/BoardingPermissionType</rdfs:comment>
        <rdfs:comment xml:lang="en">This property describes the types of boarding permissions allowed for an Onboard Stay from the SKOS codelist for types of facilities, including normal, early boarding, late alighting, etc.</rdfs:comment>
        <rdfs:label xml:lang="en">boarding permission</rdfs:label>
    </owl:ObjectProperty>
    


    <!-- https://w3id.org/transmodel/facilities#checkConstraint -->

    <owl:ObjectProperty rdf:about="https://w3id.org/transmodel/facilities#checkConstraint">
        <rdfs:subPropertyOf rdf:resource="https://w3id.org/transmodel/facilities#OBJECTPROPERTIESTOREVIEW"/>
        <rdfs:domain rdf:resource="https://w3id.org/transmodel/facilities#SiteComponent"/>
        <rdfs:range rdf:resource="https://w3id.org/transmodel/facilities#Constraint"/>
        <rdfs:label xml:lang="en">siteComponentCheckConstraint</rdfs:label>
    </owl:ObjectProperty>
    


    <!-- https://w3id.org/transmodel/facilities#comprises -->

    <owl:ObjectProperty rdf:about="https://w3id.org/transmodel/facilities#comprises">
        <rdfs:comment xml:lang="en">General property for all types of containment and aggregation</rdfs:comment>
        <rdfs:label xml:lang="en">comprises</rdfs:label>
    </owl:ObjectProperty>
    


    <!-- https://w3id.org/transmodel/facilities#comprisesEquipment -->

    <owl:ObjectProperty rdf:about="https://w3id.org/transmodel/facilities#comprisesEquipment">
        <rdfs:subPropertyOf rdf:resource="https://w3id.org/transmodel/facilities#comprises"/>
        <rdfs:domain rdf:resource="https://w3id.org/transmodel/facilities#FacilitySet"/>
        <rdfs:range rdf:resource="https://w3id.org/transmodel/facilities#Equipment"/>
        <rdfs:comment xml:lang="en">TODO: Check carefully whether the range should be Equipment or, instead, something more general like Facility, since the differentiation between Facility and Equipment is sometimes unclear</rdfs:comment>
        <rdfs:comment xml:lang="en">This property is used to aggregate other types of facilities from a Facility Set, normally focused on those that are user defined and not from the predefined list.
In the Transmodel UML model this is represented as TypeOfEquipment, and in the Netex implementation the term otherFacilities is used.</rdfs:comment>
        <rdfs:label xml:lang="en">comprises equipment</rdfs:label>
    </owl:ObjectProperty>
    


    <!-- https://w3id.org/transmodel/facilities#comprisesFacility -->

    <owl:ObjectProperty rdf:about="https://w3id.org/transmodel/facilities#comprisesFacility">
        <rdfs:subPropertyOf rdf:resource="https://w3id.org/transmodel/facilities#comprises"/>
        <rdfs:domain rdf:resource="https://w3id.org/transmodel/facilities#FacilitySet"/>
        <rdfs:range rdf:resource="https://w3id.org/transmodel/facilities#Facility"/>
        <rdfs:comment xml:lang="en">This property is used to aggregate all the facilities that a facility set contains
In Netex, this is expressed with the element TypeOfFacilityRef, which is used to refer to facilities, and in the Transmodel UML ontology this is simply expressed as &apos;facility&apos;</rdfs:comment>
        <rdfs:label xml:lang="en">comprises facility</rdfs:label>
    </owl:ObjectProperty>
    


    <!-- https://w3id.org/transmodel/facilities#concernedBy -->

    <owl:ObjectProperty rdf:about="https://w3id.org/transmodel/facilities#concernedBy">
        <rdfs:range rdf:resource="https://w3id.org/transmodel/facilities#FacilitySet"/>
        <rdfs:comment xml:lang="en">This property allows connecting any object with a Facility Set</rdfs:comment>
        <rdfs:label xml:lang="en">concerned By</rdfs:label>
    </owl:ObjectProperty>
    


    <!-- https://w3id.org/transmodel/facilities#containing -->

    <owl:ObjectProperty rdf:about="https://w3id.org/transmodel/facilities#containing">
        <rdfs:comment xml:lang="en">This property allows specifying that a Stop contains Quays</rdfs:comment>
        <rdfs:label xml:lang="en">containing</rdfs:label>
    </owl:ObjectProperty>
    


    <!-- https://w3id.org/transmodel/facilities#couchetteFacility -->

    <owl:ObjectProperty rdf:about="https://w3id.org/transmodel/facilities#couchetteFacility">
        <rdfs:subPropertyOf rdf:resource="https://w3id.org/transmodel/facilities#facilityType"/>
        <rdfs:domain rdf:resource="https://w3id.org/transmodel/facilities#Accommodation"/>
        <rdfs:range>
            <owl:Class>
                <owl:intersectionOf rdf:parseType="Collection">
                    <rdf:Description rdf:about="http://www.w3.org/2004/02/skos/core#Concept"/>
                    <owl:Restriction>
                        <owl:onProperty rdf:resource="http://www.w3.org/2004/02/skos/core#inScheme"/>
                        <owl:hasValue rdf:resource="https://w3id.org/transmodel/kos/facilities/FacilityType"/>
                    </owl:Restriction>
                </owl:intersectionOf>
            </owl:Class>
        </rdfs:range>
        <rdfs:comment xml:lang="en">TODO: the range of this property may be further restricted to those SKOS concepts that also comply with skos:broader tmkosfacility:FacilityType/CouchetteFacilityType</rdfs:comment>
        <rdfs:comment xml:lang="en">This property restricts the type of facility to one specific for couchette from the SKOS codelist for types of facilities, including, for example, values like T2, T3, C1, C2, etc.</rdfs:comment>
        <rdfs:label xml:lang="en">couchette facility</rdfs:label>
    </owl:ObjectProperty>
    


    <!-- https://w3id.org/transmodel/facilities#determining -->

    <owl:ObjectProperty rdf:about="https://w3id.org/transmodel/facilities#determining">
        <rdfs:domain rdf:resource="https://w3id.org/transmodel/facilities#AccessibilityAssessment"/>
        <rdfs:range rdf:resource="https://w3id.org/transmodel/facilities#AccessibilityLimitation"/>
        <rdfs:comment xml:lang="en">This property sets the relationship between Accessibility Assessment and Accessibility Limitation</rdfs:comment>
        <rdfs:label xml:lang="en">determining</rdfs:label>
    </owl:ObjectProperty>
    


    <!-- https://w3id.org/transmodel/facilities#displayAssignment -->

    <owl:ObjectProperty rdf:about="https://w3id.org/transmodel/facilities#displayAssignment">
        <rdfs:subPropertyOf rdf:resource="https://w3id.org/transmodel/facilities#OBJECTPROPERTIESTOREVIEW"/>
        <rdfs:domain rdf:resource="https://w3id.org/transmodel/facilities#JourneyPattern"/>
        <rdfs:comment xml:lang="en">The assignment of one ScheduledStopPoint and one JourneyPattern to a PassengerInformationEquipment specifying that information on the ScheduledStopPoint and the JourneyPattern will be provided (e.g. displayed, printed)</rdfs:comment>
        <rdfs:label xml:lang="en">displayAssignment</rdfs:label>
    </owl:ObjectProperty>
    


    <!-- https://w3id.org/transmodel/facilities#equipmentType -->

    <owl:ObjectProperty rdf:about="https://w3id.org/transmodel/facilities#equipmentType">
        <rdfs:subPropertyOf rdf:resource="http://www.w3.org/2002/07/owl#topObjectProperty"/>
        <rdfs:domain rdf:resource="https://w3id.org/transmodel/facilities#Equipment"/>
        <rdfs:range>
            <owl:Class>
                <owl:intersectionOf rdf:parseType="Collection">
                    <rdf:Description rdf:about="http://www.w3.org/2004/02/skos/core#Concept"/>
                    <owl:Restriction>
                        <owl:onProperty rdf:resource="http://www.w3.org/2004/02/skos/core#inScheme"/>
                        <owl:hasValue rdf:resource="https://w3id.org/transmodel/kos/facilities/EquipmentType"/>
                    </owl:Restriction>
                </owl:intersectionOf>
            </owl:Class>
        </rdfs:range>
        <rdfs:comment xml:lang="en">This property is used to link an equipment with the types of equipments available in the SKOS concept scheme of types of equipments</rdfs:comment>
        <rdfs:label xml:lang="en">equipment Type</rdfs:label>
    </owl:ObjectProperty>
    


    <!-- https://w3id.org/transmodel/facilities#equippedWith -->

    <owl:ObjectProperty rdf:about="https://w3id.org/transmodel/facilities#equippedWith">
        <rdfs:domain rdf:resource="https://w3id.org/transmodel/facilities#EquipmentPlace"/>
        <rdfs:range rdf:resource="https://w3id.org/transmodel/facilities#Equipment"/>
        <rdfs:comment xml:lang="en">TODO: relate it to a more general property for containment and partOf</rdfs:comment>
        <rdfs:comment xml:lang="en">This property is used to define the equipments that are available in an equipment place</rdfs:comment>
        <rdfs:label xml:lang="en">equipped With</rdfs:label>
    </owl:ObjectProperty>
    


    <!-- https://w3id.org/transmodel/facilities#facilityRequirement -->

    <owl:ObjectProperty rdf:about="https://w3id.org/transmodel/facilities#facilityRequirement">
        <rdfs:subPropertyOf rdf:resource="https://w3id.org/transmodel/facilities#OBJECTPROPERTIESTOREVIEW"/>
        <rdfs:domain rdf:resource="https://w3id.org/transmodel/facilities#Vehicle"/>
        <rdfs:range rdf:resource="https://w3id.org/transmodel/facilities#Facility"/>
        <rdfs:comment xml:lang="en">A classification of public transport Vehicles according to the facilities available on the Vehicle</rdfs:comment>
        <rdfs:label xml:lang="en">facilityRequirement</rdfs:label>
    </owl:ObjectProperty>
    


    <!-- https://w3id.org/transmodel/facilities#facilitySet -->

    <owl:ObjectProperty rdf:about="https://w3id.org/transmodel/facilities#facilitySet">
        <rdfs:subPropertyOf rdf:resource="https://w3id.org/transmodel/facilities#OBJECTPROPERTIESTOREVIEW"/>
        <rdfs:comment xml:lang="en">Set of Facilities available for a ServiceJourney or a JourneyPart. The set may be available only for a specific VehicleType within the service (e.g. carriage equipped with low floor)</rdfs:comment>
        <rdfs:label xml:lang="en">facilitySet</rdfs:label>
    </owl:ObjectProperty>
    


    <!-- https://w3id.org/transmodel/facilities#facilityType -->

    <owl:ObjectProperty rdf:about="https://w3id.org/transmodel/facilities#facilityType">
        <rdfs:domain rdf:resource="https://w3id.org/transmodel/facilities#Facility"/>
        <rdfs:range>
            <owl:Class>
                <owl:intersectionOf rdf:parseType="Collection">
                    <rdf:Description rdf:about="http://www.w3.org/2004/02/skos/core#Concept"/>
                    <owl:Restriction>
                        <owl:onProperty rdf:resource="http://www.w3.org/2004/02/skos/core#inScheme"/>
                        <owl:hasValue rdf:resource="https://w3id.org/transmodel/kos/facilities/FacilityType"/>
                    </owl:Restriction>
                </owl:intersectionOf>
            </owl:Class>
        </rdfs:range>
        <rdfs:comment xml:lang="en">This property is used to link a facility with the types of facilities available in the SKOS concept scheme of types of facilities</rdfs:comment>
        <rdfs:comment xml:lang="en">facility type</rdfs:comment>
    </owl:ObjectProperty>
    


    <!-- https://w3id.org/transmodel/facilities#fareClass -->

    <owl:ObjectProperty rdf:about="https://w3id.org/transmodel/facilities#fareClass">
        <rdfs:subPropertyOf rdf:resource="https://w3id.org/transmodel/facilities#facilityType"/>
        <rdfs:domain rdf:resource="https://w3id.org/transmodel/facilities#ServiceFacilitySet"/>
        <rdfs:range>
            <owl:Class>
                <owl:intersectionOf rdf:parseType="Collection">
                    <rdf:Description rdf:about="http://www.w3.org/2004/02/skos/core#Concept"/>
                    <owl:Restriction>
                        <owl:onProperty rdf:resource="http://www.w3.org/2004/02/skos/core#inScheme"/>
                        <owl:hasValue rdf:resource="https://w3id.org/transmodel/kos/facilities/FacilityType"/>
                    </owl:Restriction>
                </owl:intersectionOf>
            </owl:Class>
        </rdfs:range>
        <rdfs:comment xml:lang="en">TODO: create the list of allowed values for fare classes, and check whether including it as a facility type, as included in the TransModel model</rdfs:comment>
        <rdfs:comment xml:lang="en">This property relates an Onboard Stay or an Accommodation, among others, with a class of fares, whose allowed values are defined in the TransModel Common Facility Values (Figure 290, page 454)</rdfs:comment>
        <rdfs:label xml:lang="en">fare class</rdfs:label>
    </owl:ObjectProperty>
    


    <!-- https://w3id.org/transmodel/facilities#isUsedBy -->

    <owl:ObjectProperty rdf:about="https://w3id.org/transmodel/facilities#isUsedBy">
        <rdfs:subPropertyOf rdf:resource="https://w3id.org/transmodel/facilities#OBJECTPROPERTIESTOREVIEW"/>
        <rdfs:domain rdf:resource="https://w3id.org/transmodel/facilities#Facility"/>
        <rdfs:range rdf:resource="https://w3id.org/transmodel/facilities#Passenger"/>
        <rdfs:label xml:lang="en">isUsedBy</rdfs:label>
    </owl:ObjectProperty>
    


    <!-- https://w3id.org/transmodel/facilities#locatedIn -->

    <owl:ObjectProperty rdf:about="https://w3id.org/transmodel/facilities#locatedIn">
        <rdfs:domain rdf:resource="https://w3id.org/transmodel/facilities#Equipment"/>
        <rdfs:range rdf:resource="https://w3id.org/transmodel/facilities#EquipmentPlace"/>
        <rdfs:comment xml:lang="en">TODO: find a more general property (probably similar to contains/containedIn) and think about whether it should be replaced by this more general property, or at least created as a subProperty of that one.</rdfs:comment>
        <rdfs:comment xml:lang="en">This property is used to relate an equipment with the equipment place where it is located</rdfs:comment>
        <rdfs:label xml:lang="en">located In</rdfs:label>
    </owl:ObjectProperty>
    


    <!-- https://w3id.org/transmodel/facilities#noticeAssignment -->

    <owl:ObjectProperty rdf:about="https://w3id.org/transmodel/facilities#noticeAssignment">
        <rdfs:subPropertyOf rdf:resource="https://w3id.org/transmodel/facilities#OBJECTPROPERTIESTOREVIEW"/>
        <rdfs:domain rdf:resource="https://w3id.org/transmodel/facilities#JourneyPattern"/>
        <rdfs:range rdf:resource="https://w3id.org/transmodel/facilities#Notice"/>
        <rdfs:comment xml:lang="en">The assignment of a Notice showing an exception in a JourneyPattern, a CommonSection or a VehicleJourney, possibly specifying at which PointInJourneyPattern the validity of the Notice starts and ends respectively</rdfs:comment>
        <rdfs:label xml:lang="en">noticeAssignment</rdfs:label>
    </owl:ObjectProperty>
    


    <!-- https://w3id.org/transmodel/facilities#position -->

    <owl:ObjectProperty rdf:about="https://w3id.org/transmodel/facilities#position">
        <rdfs:domain>
            <owl:Class>
                <owl:unionOf rdf:parseType="Collection">
                    <rdf:Description rdf:about="https://w3id.org/transmodel/facilities#EquipmentPlace"/>
                    <rdf:Description rdf:about="https://w3id.org/transmodel/facilities#PlaceEquipment"/>
                </owl:unionOf>
            </owl:Class>
        </rdfs:domain>
        <rdfs:range rdf:resource="https://w3id.org/transmodel/facilities#EquipmentPosition"/>
        <rdfs:comment xml:lang="en">This property is used to relate an equipment place (a collection of equipments) or a specific place equipment with the different equipment positions that they may have</rdfs:comment>
        <rdfs:label xml:lang="en">position</rdfs:label>
    </owl:ObjectProperty>
    


    <!-- https://w3id.org/transmodel/facilities#presentAt -->

    <owl:ObjectProperty rdf:about="https://w3id.org/transmodel/facilities#presentAt">
        <rdfs:domain rdf:resource="https://w3id.org/transmodel/facilities#ServiceFacilitySet"/>
        <rdfs:range rdf:resource="https://w3id.org/transmodel/facilities#VehicleType"/>
        <rdfs:comment xml:lang="en">This property relates a Service Facility Set with a Vehicle Type, indicating that the set of service facilities comprised by the set are provided at that type of vehicle</rdfs:comment>
        <rdfs:label xml:lang="en">present at</rdfs:label>
    </owl:ObjectProperty>
    


    <!-- https://w3id.org/transmodel/facilities#providedBy -->

    <owl:ObjectProperty rdf:about="https://w3id.org/transmodel/facilities#providedBy">
        <rdfs:subPropertyOf rdf:resource="http://www.w3.org/2002/07/owl#topObjectProperty"/>
        <rdfs:domain rdf:resource="https://w3id.org/transmodel/facilities#FacilitySet"/>
        <rdfs:comment xml:lang="es">TODO: Add org:Organization as range for this property
TODO: Check whether the domain should be generalised (applicable not only to facility set but also to facility, site, equipment, etc.)</rdfs:comment>
        <rdfs:comment xml:lang="es">This property is used to refer to the provider of a facility set
In the TransModel UML model and in the Netex implementation this is expressed as ProvidedByRef</rdfs:comment>
        <rdfs:label xml:lang="es">provided by</rdfs:label>
    </owl:ObjectProperty>
    


    <!-- https://w3id.org/transmodel/facilities#showerFacility -->

    <owl:ObjectProperty rdf:about="https://w3id.org/transmodel/facilities#showerFacility">
        <rdfs:subPropertyOf rdf:resource="https://w3id.org/transmodel/facilities#facilityType"/>
        <rdfs:domain rdf:resource="https://w3id.org/transmodel/facilities#Accommodation"/>
        <rdfs:range>
            <owl:Class>
                <owl:intersectionOf rdf:parseType="Collection">
                    <rdf:Description rdf:about="http://www.w3.org/2004/02/skos/core#Concept"/>
                    <owl:Restriction>
                        <owl:onProperty rdf:resource="http://www.w3.org/2004/02/skos/core#inScheme"/>
                        <owl:hasValue rdf:resource="https://w3id.org/transmodel/kos/facilities/FacilityType"/>
                    </owl:Restriction>
                </owl:intersectionOf>
            </owl:Class>
        </rdfs:range>
        <rdfs:comment xml:lang="en">TODO: the range of this property may be further restricted to those SKOS concepts that also comply with skos:broader tmkosfacility:FacilityType/XXX, where XXX refers to the shower facilities</rdfs:comment>
        <rdfs:comment xml:lang="en">This property restricts the type of facility to one specific for shower from the SKOS codelist for types of facilities. However, there is no specific part of the codelist reserved yet for shower facilities.</rdfs:comment>
        <rdfs:label xml:lang="en">shower facility</rdfs:label>
    </owl:ObjectProperty>
    


    <!-- https://w3id.org/transmodel/facilities#stopPlaceComponent -->

    <owl:ObjectProperty rdf:about="https://w3id.org/transmodel/facilities#stopPlaceComponent">
        <rdfs:subPropertyOf rdf:resource="https://w3id.org/transmodel/facilities#OBJECTPROPERTIESTOREVIEW"/>
        <rdfs:range rdf:resource="https://w3id.org/transmodel/facilities#StopPlaceComponent"/>
        <rdfs:label xml:lang="en">stopPlaceComponent</rdfs:label>
    </owl:ObjectProperty>
    


    <!-- https://w3id.org/transmodel/facilities#stopPlaceEntrance -->

    <owl:ObjectProperty rdf:about="https://w3id.org/transmodel/facilities#stopPlaceEntrance">
        <rdfs:subPropertyOf rdf:resource="https://w3id.org/transmodel/facilities#OBJECTPROPERTIESTOREVIEW"/>
        <rdfs:range rdf:resource="https://w3id.org/transmodel/facilities#AccessEquipment"/>
        <rdfs:comment xml:lang="en">A physical entrance or exit to/from a StopPlace for a Passenger. May be a door, barrier, gate other recognizable point of access</rdfs:comment>
        <rdfs:comment xml:lang="en">stopPlaceEntrance</rdfs:comment>
    </owl:ObjectProperty>
    


    <!-- https://w3id.org/transmodel/facilities#subplaceOf -->

    <owl:ObjectProperty rdf:about="https://w3id.org/transmodel/facilities#subplaceOf">
        <rdfs:domain rdf:resource="https://w3id.org/transmodel/facilities#StopPlace"/>
        <rdfs:range rdf:resource="https://w3id.org/transmodel/facilities#StopPlace"/>
        <rdfs:comment xml:lang="en">A property connecting one Stop Place to another Stop Place to describe nested Stop Places (e.g. a metro station in a train station).</rdfs:comment>
        <rdfs:label xml:lang="en">subplace of</rdfs:label>
    </owl:ObjectProperty>
    


    <!-- https://w3id.org/transmodel/facilities#toiletFacility -->

    <owl:ObjectProperty rdf:about="https://w3id.org/transmodel/facilities#toiletFacility">
        <rdfs:subPropertyOf rdf:resource="https://w3id.org/transmodel/facilities#facilityType"/>
        <rdfs:domain rdf:resource="https://w3id.org/transmodel/facilities#Accommodation"/>
        <rdfs:range>
            <owl:Class>
                <owl:intersectionOf rdf:parseType="Collection">
                    <rdf:Description rdf:about="http://www.w3.org/2004/02/skos/core#Concept"/>
                    <owl:Restriction>
                        <owl:onProperty rdf:resource="http://www.w3.org/2004/02/skos/core#inScheme"/>
                        <owl:hasValue rdf:resource="https://w3id.org/transmodel/kos/facilities/FacilityType"/>
                    </owl:Restriction>
                </owl:intersectionOf>
            </owl:Class>
        </rdfs:range>
        <rdfs:comment xml:lang="en">TODO: the range of this property may be further restricted to those SKOS concepts that also comply with skos:broader tmkosfacility:FacilityType/XXX, where XXX refers to the toilet facilities</rdfs:comment>
        <rdfs:comment xml:lang="en">This property restricts the type of facility to one specific for toilets from the SKOS codelist for types of facilities. However, there is no specific part of the codelist reserved yet for toilet facilities (also known as sanitary facilities).</rdfs:comment>
        <rdfs:label xml:lang="en">toilet facility</rdfs:label>
    </owl:ObjectProperty>
    


    <!-- https://w3id.org/transmodel/facilities#typeOfAccessFeature -->

    <owl:ObjectProperty rdf:about="https://w3id.org/transmodel/facilities#typeOfAccessFeature">
        <rdfs:subPropertyOf rdf:resource="https://w3id.org/transmodel/facilities#OBJECTPROPERTIESTOREVIEW"/>
        <rdfs:domain rdf:resource="https://w3id.org/transmodel/facilities#ConstraintOfAccess"/>
    </owl:ObjectProperty>
    


    <!-- https://w3id.org/transmodel/facilities#typeOfAccessibilityTools -->

    <owl:ObjectProperty rdf:about="https://w3id.org/transmodel/facilities#typeOfAccessibilityTools">
        <rdfs:subPropertyOf rdf:resource="https://w3id.org/transmodel/facilities#OBJECTPROPERTIESTOREVIEW"/>
        <rdfs:domain rdf:resource="https://w3id.org/transmodel/facilities#AssistanceService"/>
        <rdfs:label xml:lang="en">typeOfAccessibilityTools</rdfs:label>
    </owl:ObjectProperty>
    


    <!-- https://w3id.org/transmodel/facilities#typeOfCateringService -->

    <owl:ObjectProperty rdf:about="https://w3id.org/transmodel/facilities#typeOfCateringService">
        <rdfs:subPropertyOf rdf:resource="https://w3id.org/transmodel/facilities#OBJECTPROPERTIESTOREVIEW"/>
        <rdfs:domain rdf:resource="https://w3id.org/transmodel/facilities#CateringService"/>
        <rdfs:label xml:lang="en">typeOfCateringService</rdfs:label>
    </owl:ObjectProperty>
    


    <!-- https://w3id.org/transmodel/facilities#typeOfCheckConstraint -->

    <owl:ObjectProperty rdf:about="https://w3id.org/transmodel/facilities#typeOfCheckConstraint">
        <rdfs:subPropertyOf rdf:resource="https://w3id.org/transmodel/facilities#OBJECTPROPERTIESTOREVIEW"/>
        <rdfs:domain rdf:resource="https://w3id.org/transmodel/facilities#Constraint"/>
        <rdfs:label xml:lang="en">typeOfCheckConstraint</rdfs:label>
    </owl:ObjectProperty>
    


    <!-- https://w3id.org/transmodel/facilities#typeOfCongestion -->

    <owl:ObjectProperty rdf:about="https://w3id.org/transmodel/facilities#typeOfCongestion">
        <rdfs:subPropertyOf rdf:resource="https://w3id.org/transmodel/facilities#OBJECTPROPERTIESTOREVIEW"/>
        <rdfs:label xml:lang="en">typeOfCongestion</rdfs:label>
    </owl:ObjectProperty>
    


    <!-- https://w3id.org/transmodel/facilities#typeOfCycleEquipment -->

    <owl:ObjectProperty rdf:about="https://w3id.org/transmodel/facilities#typeOfCycleEquipment">
        <rdfs:subPropertyOf rdf:resource="https://w3id.org/transmodel/facilities#OBJECTPROPERTIESTOREVIEW"/>
        <rdfs:domain rdf:resource="https://w3id.org/transmodel/facilities#CycleOperatingEquipment"/>
        <rdfs:label>typeOfCycleStorageEquipment</rdfs:label>
    </owl:ObjectProperty>
    


    <!-- https://w3id.org/transmodel/facilities#typeOfEmergencyService -->

    <owl:ObjectProperty rdf:about="https://w3id.org/transmodel/facilities#typeOfEmergencyService">
        <rdfs:subPropertyOf rdf:resource="https://w3id.org/transmodel/facilities#OBJECTPROPERTIESTOREVIEW"/>
        <rdfs:domain rdf:resource="https://w3id.org/transmodel/facilities#EmergencyService"/>
        <rdfs:label xml:lang="en">typeOfEmergencyService</rdfs:label>
    </owl:ObjectProperty>
    


    <!-- https://w3id.org/transmodel/facilities#typeOfEntranceEquipment -->

    <owl:ObjectProperty rdf:about="https://w3id.org/transmodel/facilities#typeOfEntranceEquipment">
        <rdfs:subPropertyOf rdf:resource="https://w3id.org/transmodel/facilities#OBJECTPROPERTIESTOREVIEW"/>
        <rdfs:domain rdf:resource="https://w3id.org/transmodel/facilities#EntranceEquipment"/>
        <rdfs:comment xml:lang="en">Classification of the Entrance Equipment</rdfs:comment>
        <rdfs:label xml:lang="en">typeOfEntranceEquipment</rdfs:label>
    </owl:ObjectProperty>
    


    <!-- https://w3id.org/transmodel/facilities#typeOfGenderLimitation -->

    <owl:ObjectProperty rdf:about="https://w3id.org/transmodel/facilities#typeOfGenderLimitation">
        <rdfs:subPropertyOf rdf:resource="https://w3id.org/transmodel/facilities#OBJECTPROPERTIESTOREVIEW"/>
        <rdfs:domain rdf:resource="https://w3id.org/transmodel/facilities#SanitaryEquipment"/>
        <rdfs:label xml:lang="en">typeOfGenderLimitation</rdfs:label>
    </owl:ObjectProperty>
    


    <!-- https://w3id.org/transmodel/facilities#typeOfHandrail -->

    <owl:ObjectProperty rdf:about="https://w3id.org/transmodel/facilities#typeOfHandrail">
        <rdfs:subPropertyOf rdf:resource="https://w3id.org/transmodel/facilities#OBJECTPROPERTIESTOREVIEW"/>
        <rdfs:domain rdf:resource="https://w3id.org/transmodel/facilities#StairEquipment"/>
        <rdfs:comment>types of handrails</rdfs:comment>
        <rdfs:label xml:lang="en">typeOfHandrail</rdfs:label>
    </owl:ObjectProperty>
    


    <!-- https://w3id.org/transmodel/facilities#typeOfPassengerInformationDesk -->

    <owl:ObjectProperty rdf:about="https://w3id.org/transmodel/facilities#typeOfPassengerInformationDesk">
        <rdfs:subPropertyOf rdf:resource="https://w3id.org/transmodel/facilities#OBJECTPROPERTIESTOREVIEW"/>
        <rdfs:domain rdf:resource="https://w3id.org/transmodel/facilities#PassengerInformationEquipment"/>
        <rdfs:comment xml:lang="en">The relationship between the PassengerInformationDesk with the typeOfInformationDesk</rdfs:comment>
        <rdfs:label xml:lang="en">typeOfPassengerInformationDesk</rdfs:label>
    </owl:ObjectProperty>
    


    <!-- https://w3id.org/transmodel/facilities#typeOfPlaceAccessStair -->

    <owl:ObjectProperty rdf:about="https://w3id.org/transmodel/facilities#typeOfPlaceAccessStair">
        <rdfs:subPropertyOf rdf:resource="https://w3id.org/transmodel/facilities#OBJECTPROPERTIESTOREVIEW"/>
        <rdfs:domain rdf:resource="https://w3id.org/transmodel/facilities#StairEquipment"/>
        <rdfs:label xml:lang="en">typeOfPlaceAccessStairs</rdfs:label>
    </owl:ObjectProperty>
    


    <!-- https://w3id.org/transmodel/facilities#typeOfSanitaryEquipment -->

    <owl:ObjectProperty rdf:about="https://w3id.org/transmodel/facilities#typeOfSanitaryEquipment">
        <rdfs:subPropertyOf rdf:resource="https://w3id.org/transmodel/facilities#OBJECTPROPERTIESTOREVIEW"/>
        <rdfs:range rdf:resource="https://w3id.org/transmodel/facilities#SanitaryEquipment"/>
        <rdfs:label xml:lang="en">typeOfSanitaryEquipment</rdfs:label>
    </owl:ObjectProperty>
    


    <!-- https://w3id.org/transmodel/facilities#typeOfVehicle -->

    <owl:ObjectProperty rdf:about="https://w3id.org/transmodel/facilities#typeOfVehicle">
        <rdfs:subPropertyOf rdf:resource="https://w3id.org/transmodel/facilities#OBJECTPROPERTIESTOREVIEW"/>
        <rdfs:domain rdf:resource="https://w3id.org/transmodel/facilities#Vehicle"/>
        <rdfs:range rdf:resource="https://w3id.org/transmodel/facilities#VehicleType"/>
        <rdfs:label xml:lang="en">typeOfVehicle</rdfs:label>
    </owl:ObjectProperty>
    


    <!-- https://w3id.org/transmodel/facilities#typeOfWaitingRoom -->

    <owl:ObjectProperty rdf:about="https://w3id.org/transmodel/facilities#typeOfWaitingRoom">
        <rdfs:subPropertyOf rdf:resource="https://w3id.org/transmodel/facilities#OBJECTPROPERTIESTOREVIEW"/>
        <rdfs:domain rdf:resource="https://w3id.org/transmodel/facilities#WaitingRoomEquipment"/>
        <rdfs:label xml:lang="en">typeOfWaitingRoomEquipment</rdfs:label>
    </owl:ObjectProperty>
    


    <!-- https://w3id.org/transmodel/facilities#userNeedSuitability -->

    <owl:ObjectProperty rdf:about="https://w3id.org/transmodel/facilities#userNeedSuitability">
        <rdfs:subPropertyOf rdf:resource="https://w3id.org/transmodel/facilities#OBJECTPROPERTIESTOREVIEW"/>
        <rdfs:domain rdf:resource="https://w3id.org/transmodel/facilities#UserNeed"/>
        <rdfs:range rdf:resource="https://w3id.org/transmodel/facilities#Suitability"/>
        <rdfs:label xml:lang="en">userNeedSuitability</rdfs:label>
    </owl:ObjectProperty>
    


    <!-- https://w3id.org/transmodel/facilities#validityConditionDefines -->

    <owl:ObjectProperty rdf:about="https://w3id.org/transmodel/facilities#validityConditionDefines">
        <rdfs:subPropertyOf rdf:resource="https://w3id.org/transmodel/facilities#OBJECTPROPERTIESTOREVIEW"/>
        <rdfs:domain rdf:resource="https://w3id.org/transmodel/facilities#ValidityCondition"/>
        <rdfs:range rdf:resource="https://w3id.org/transmodel/facilities#ValidityTrigger"/>
        <rdfs:label xml:lang="en">validityConditionDefines</rdfs:label>
    </owl:ObjectProperty>
    


    <!-- https://w3id.org/transmodel/facilities#wheelchairAccess -->

    <owl:ObjectProperty rdf:about="https://w3id.org/transmodel/facilities#wheelchairAccess">
        <rdfs:domain rdf:resource="https://w3id.org/transmodel/facilities#AccessibilityLimitation"/>
        <rdfs:range>
            <owl:Class>
                <owl:intersectionOf rdf:parseType="Collection">
                    <rdf:Description rdf:about="http://www.w3.org/2004/02/skos/core#Concept"/>
                    <owl:Restriction>
                        <owl:onProperty rdf:resource="http://www.w3.org/2004/02/skos/core#inScheme"/>
                        <owl:hasValue rdf:resource="https://w3id.org/transmodel/kos/journeys/mobility-limitation"/>
                    </owl:Restriction>
                </owl:intersectionOf>
            </owl:Class>
        </rdfs:range>
        <rdfs:comment xml:lang="en">This property sets the relationaship between Accessibility Limitation and the kos wheelchair-access</rdfs:comment>
        <rdfs:label xml:lang="en">wheelchair Access</rdfs:label>
    </owl:ObjectProperty>
    


    <!-- https://w3id.org/transmodel/journeys#hasAServiceJourneyPattern -->

    <owl:ObjectProperty rdf:about="https://w3id.org/transmodel/journeys#hasAServiceJourneyPattern">
        <rdfs:subPropertyOf rdf:resource="https://w3id.org/transmodel/facilities#OBJECTPROPERTIESTOREVIEW"/>
        <rdfs:domain rdf:resource="https://w3id.org/transmodel/journeys#Service"/>
    </owl:ObjectProperty>
    


    <!-- https://w3id.org/transmodel/journeys#makesAServiceJourney -->

    <owl:ObjectProperty rdf:about="https://w3id.org/transmodel/journeys#makesAServiceJourney">
        <rdfs:subPropertyOf rdf:resource="https://w3id.org/transmodel/facilities#OBJECTPROPERTIESTOREVIEW"/>
        <rdfs:range rdf:resource="https://w3id.org/transmodel/journeys#Service"/>
    </owl:ObjectProperty>
    


    <!-- 
    ///////////////////////////////////////////////////////////////////////////////////////
    //
    // Data properties
    //
    ///////////////////////////////////////////////////////////////////////////////////////
     -->

    


    <!-- https://w3id.org/transmodel/commons#borderCrossing -->

    <owl:DatatypeProperty rdf:about="https://w3id.org/transmodel/commons#borderCrossing"/>
    


    <!-- https://w3id.org/transmodel/facilities#DATAPROPERTIESTOREVIEW -->

    <owl:DatatypeProperty rdf:about="https://w3id.org/transmodel/facilities#DATAPROPERTIESTOREVIEW"/>
    


    <!-- https://w3id.org/transmodel/facilities#accessDimensions -->

    <owl:DatatypeProperty rdf:about="https://w3id.org/transmodel/facilities#accessDimensions">
        <rdfs:subPropertyOf rdf:resource="https://w3id.org/transmodel/facilities#DATAPROPERTIESTOREVIEW"/>
        <rdfs:domain rdf:resource="https://w3id.org/transmodel/facilities#WheelchairVehicleEquipment"/>
        <rdfs:range rdf:resource="http://www.w3.org/2000/01/rdf-schema#Literal"/>
    </owl:DatatypeProperty>
    


    <!-- https://w3id.org/transmodel/facilities#activatedEquipment -->

    <owl:DatatypeProperty rdf:about="https://w3id.org/transmodel/facilities#activatedEquipment">
        <rdfs:subPropertyOf rdf:resource="https://w3id.org/transmodel/facilities#DATAPROPERTIESTOREVIEW"/>
        <rdfs:domain rdf:resource="https://w3id.org/transmodel/facilities#Facility"/>
        <rdfs:range rdf:resource="http://www.w3.org/2001/XMLSchema#boolean"/>
        <rdfs:label xml:lang="en">activatedEquipment</rdfs:label>
    </owl:DatatypeProperty>
    


    <!-- https://w3id.org/transmodel/facilities#constraintThroughput -->

    <owl:DatatypeProperty rdf:about="https://w3id.org/transmodel/facilities#constraintThroughput">
        <rdfs:subPropertyOf rdf:resource="https://w3id.org/transmodel/facilities#DATAPROPERTIESTOREVIEW"/>
        <rdfs:domain rdf:resource="https://w3id.org/transmodel/facilities#ConstraintThroughput"/>
        <rdfs:range rdf:resource="http://www.w3.org/2001/XMLSchema#integer"/>
        <rdfs:label xml:lang="en">constraintThroughtput</rdfs:label>
    </owl:DatatypeProperty>
    


    <!-- https://w3id.org/transmodel/facilities#duration -->

    <owl:DatatypeProperty rdf:about="https://w3id.org/transmodel/facilities#duration">
        <rdfs:domain rdf:resource="https://w3id.org/transmodel/facilities#OnboardStay"/>
        <rdfs:range rdf:resource="http://www.w3.org/2001/XMLSchema#duration"/>
        <rdfs:comment xml:lang="en">This property relates an Onboard Stay with a duration</rdfs:comment>
        <rdfs:label xml:lang="en">duration</rdfs:label>
    </owl:DatatypeProperty>
    


    <!-- https://w3id.org/transmodel/facilities#facilityLocation -->

    <owl:DatatypeProperty rdf:about="https://w3id.org/transmodel/facilities#facilityLocation">
        <rdfs:subPropertyOf rdf:resource="https://w3id.org/transmodel/facilities#DATAPROPERTIESTOREVIEW"/>
        <rdfs:domain rdf:resource="https://w3id.org/transmodel/facilities#Facility"/>
        <rdfs:label>facilityLocation</rdfs:label>
    </owl:DatatypeProperty>
    


    <!-- https://w3id.org/transmodel/facilities#fixed -->

    <owl:DatatypeProperty rdf:about="https://w3id.org/transmodel/facilities#fixed">
        <rdfs:domain rdf:resource="https://w3id.org/transmodel/facilities#Equipment"/>
        <rdfs:range rdf:resource="http://www.w3.org/2001/XMLSchema#boolean"/>
        <rdfs:comment xml:lang="en">This property is used to determine whether an equipment is fixed in a place or not.</rdfs:comment>
        <rdfs:label xml:lang="en">fixed</rdfs:label>
    </owl:DatatypeProperty>
    


    <!-- https://w3id.org/transmodel/facilities#freeToUse -->

    <owl:DatatypeProperty rdf:about="https://w3id.org/transmodel/facilities#freeToUse">
        <rdfs:subPropertyOf rdf:resource="https://w3id.org/transmodel/facilities#DATAPROPERTIESTOREVIEW"/>
        <rdfs:domain rdf:resource="https://w3id.org/transmodel/facilities#LocalService"/>
        <rdfs:range rdf:resource="http://www.w3.org/2001/XMLSchema#boolean"/>
        <rdfs:comment xml:lang="en">Characteristic of a Service that is free to use it</rdfs:comment>
        <rdfs:label xml:lang="en">freeToUse</rdfs:label>
    </owl:DatatypeProperty>
    


    <!-- https://w3id.org/transmodel/facilities#outOfService -->

    <owl:DatatypeProperty rdf:about="https://w3id.org/transmodel/facilities#outOfService">
        <rdfs:domain rdf:resource="https://w3id.org/transmodel/facilities#Equipment"/>
        <rdfs:range rdf:resource="http://www.w3.org/2001/XMLSchema#boolean"/>
        <rdfs:comment xml:lang="en">This property allows specifying whether the equipment is out of service or not</rdfs:comment>
        <rdfs:label xml:lang="en">out of service</rdfs:label>
    </owl:DatatypeProperty>
    


    <!-- https://w3id.org/transmodel/facilities#siteComponentTimePenalty -->

    <owl:DatatypeProperty rdf:about="https://w3id.org/transmodel/facilities#siteComponentTimePenalty">
        <rdfs:subPropertyOf rdf:resource="https://w3id.org/transmodel/facilities#DATAPROPERTIESTOREVIEW"/>
        <rdfs:domain rdf:resource="https://w3id.org/transmodel/facilities#ConstraintDelay"/>
        <rdfs:range rdf:resource="http://www.w3.org/2001/XMLSchema#dateTime"/>
        <rdfs:label xml:lang="en">constraintDelayInterval</rdfs:label>
    </owl:DatatypeProperty>
    


    <!-- https://w3id.org/transmodel/facilities#wheelchairAreas -->

    <owl:DatatypeProperty rdf:about="https://w3id.org/transmodel/facilities#wheelchairAreas">
        <rdfs:subPropertyOf rdf:resource="https://w3id.org/transmodel/facilities#DATAPROPERTIESTOREVIEW"/>
        <rdfs:domain rdf:resource="https://w3id.org/transmodel/facilities#WheelchairVehicleEquipment"/>
        <rdfs:range rdf:resource="http://www.w3.org/2001/XMLSchema#integer"/>
    </owl:DatatypeProperty>
    


    <!-- 
    ///////////////////////////////////////////////////////////////////////////////////////
    //
    // Classes
    //
    ///////////////////////////////////////////////////////////////////////////////////////
     -->

    


    <!-- http://www.w3.org/2004/02/skos/core#Concept -->

    <owl:Class rdf:about="http://www.w3.org/2004/02/skos/core#Concept"/>
    


    <!-- http://www.w3.org/2004/02/skos/core#ConceptScheme -->

    <owl:Class rdf:about="http://www.w3.org/2004/02/skos/core#ConceptScheme"/>
    


    <!-- https://w3id.org/transmodel/facilities#AccessAreaDimensions -->

    <owl:Class rdf:about="https://w3id.org/transmodel/facilities#AccessAreaDimensions">
        <rdfs:subClassOf rdf:resource="https://w3id.org/transmodel/facilities#VehicleAccessEquipment"/>
        <rdfs:comment xml:lang="en">Specialisation of VehicleAccessEquipment dedicated to VehicleAccessAreaDimmension</rdfs:comment>
        <rdfs:comment xml:lang="en">TODO: Check if this has to be maintained, as it is not present in the Equipment Overview Physical Model of Transmodel (figure 247)</rdfs:comment>
        <rdfs:label xml:lang="en">VehicleAccessAreaDimension</rdfs:label>
    </owl:Class>
    


    <!-- https://w3id.org/transmodel/facilities#AccessEquipment -->

    <owl:Class rdf:about="https://w3id.org/transmodel/facilities#AccessEquipment">
        <rdfs:subClassOf rdf:resource="https://w3id.org/transmodel/facilities#PlaceEquipment"/>
        <rdfs:comment xml:lang="en">Specialisation of Place Equipment dedicated to access (e.g. lifts, entrances, stairs, ramps, etc.)</rdfs:comment>
        <rdfs:label xml:lang="en">Access Equipment</rdfs:label>
    </owl:Class>
    


    <!-- https://w3id.org/transmodel/facilities#AccessSpace -->

    <owl:Class rdf:about="https://w3id.org/transmodel/facilities#AccessSpace">
        <owl:equivalentClass rdf:resource="https://w3id.org/transmodel/facilities#PassengerArea"/>
        <rdfs:subClassOf rdf:resource="https://w3id.org/transmodel/facilities#THINGSTOREVIEW"/>
        <rdfs:label xml:lang="en">AccessSpace</rdfs:label>
    </owl:Class>
    


    <!-- https://w3id.org/transmodel/facilities#AccessibilityAssessment -->

    <owl:Class rdf:about="https://w3id.org/transmodel/facilities#AccessibilityAssessment">
        <rdfs:comment xml:lang="en">The accessibility characteristics of an Entity (facility)  used by Passenger such as a Stop Place or a Stop Place Component. Described by AccessibilityLimitations and/or a set of Suitabilities</rdfs:comment>
        <rdfs:label xml:lang="en">Accessibility Assessment</rdfs:label>
    </owl:Class>
    


    <!-- https://w3id.org/transmodel/facilities#AccessibilityLimitation -->

    <owl:Class rdf:about="https://w3id.org/transmodel/facilities#AccessibilityLimitation">
        <rdfs:subClassOf>
            <owl:Restriction>
                <owl:onProperty rdf:resource="https://w3id.org/transmodel/facilities#determining"/>
                <owl:allValuesFrom rdf:resource="https://w3id.org/transmodel/facilities#AccessibilityLimitation"/>
            </owl:Restriction>
        </rdfs:subClassOf>
        <rdfs:comment xml:lang="en">A categorisation of the accessibility characteristics of a Site, e.g. a Stop Place or a Stop Place Component to indicate its usability by passengers with specific needs, for example, those needing wheelchair access, step-free access or wanting to avoid confined spaces such as lifts. 
A small number of well-defined categories are used that are chosen to allow the consistent capture of data and the efficient computation of routes for different classes of user.</rdfs:comment>
        <rdfs:label xml:lang="en">Accessibility Limitation</rdfs:label>
    </owl:Class>
    


    <!-- https://w3id.org/transmodel/facilities#Accommodation -->

    <owl:Class rdf:about="https://w3id.org/transmodel/facilities#Accommodation">
        <rdfs:subClassOf rdf:resource="https://w3id.org/transmodel/facilities#Facility"/>
        <rdfs:subClassOf>
            <owl:Restriction>
                <owl:onProperty rdf:resource="https://w3id.org/transmodel/facilities#accommodationFacility"/>
                <owl:maxQualifiedCardinality rdf:datatype="http://www.w3.org/2001/XMLSchema#nonNegativeInteger">1</owl:maxQualifiedCardinality>
                <owl:onClass>
                    <owl:Class>
                        <owl:intersectionOf rdf:parseType="Collection">
                            <rdf:Description rdf:about="http://www.w3.org/2004/02/skos/core#Concept"/>
                            <owl:Restriction>
                                <owl:onProperty rdf:resource="http://www.w3.org/2004/02/skos/core#inScheme"/>
                                <owl:hasValue rdf:resource="https://w3id.org/transmodel/kos/facilities/FacilityType"/>
                            </owl:Restriction>
                        </owl:intersectionOf>
                    </owl:Class>
                </owl:onClass>
            </owl:Restriction>
        </rdfs:subClassOf>
        <rdfs:subClassOf>
            <owl:Restriction>
                <owl:onProperty rdf:resource="https://w3id.org/transmodel/facilities#couchetteFacility"/>
                <owl:maxQualifiedCardinality rdf:datatype="http://www.w3.org/2001/XMLSchema#nonNegativeInteger">1</owl:maxQualifiedCardinality>
                <owl:onClass>
                    <owl:Class>
                        <owl:intersectionOf rdf:parseType="Collection">
                            <rdf:Description rdf:about="http://www.w3.org/2004/02/skos/core#Concept"/>
                            <owl:Restriction>
                                <owl:onProperty rdf:resource="http://www.w3.org/2004/02/skos/core#inScheme"/>
                                <owl:hasValue rdf:resource="https://w3id.org/transmodel/kos/facilities/FacilityType"/>
                            </owl:Restriction>
                        </owl:intersectionOf>
                    </owl:Class>
                </owl:onClass>
            </owl:Restriction>
        </rdfs:subClassOf>
        <rdfs:subClassOf>
            <owl:Restriction>
                <owl:onProperty rdf:resource="https://w3id.org/transmodel/facilities#fareClass"/>
                <owl:maxQualifiedCardinality rdf:datatype="http://www.w3.org/2001/XMLSchema#nonNegativeInteger">1</owl:maxQualifiedCardinality>
                <owl:onClass>
                    <owl:Class>
                        <owl:intersectionOf rdf:parseType="Collection">
                            <rdf:Description rdf:about="http://www.w3.org/2004/02/skos/core#Concept"/>
                            <owl:Restriction>
                                <owl:onProperty rdf:resource="http://www.w3.org/2004/02/skos/core#inScheme"/>
                                <owl:hasValue rdf:resource="https://w3id.org/transmodel/kos/facilities/FacilityType"/>
                            </owl:Restriction>
                        </owl:intersectionOf>
                    </owl:Class>
                </owl:onClass>
            </owl:Restriction>
        </rdfs:subClassOf>
        <rdfs:subClassOf>
            <owl:Restriction>
                <owl:onProperty rdf:resource="https://w3id.org/transmodel/facilities#showerFacility"/>
                <owl:maxQualifiedCardinality rdf:datatype="http://www.w3.org/2001/XMLSchema#nonNegativeInteger">1</owl:maxQualifiedCardinality>
                <owl:onClass>
                    <owl:Class>
                        <owl:intersectionOf rdf:parseType="Collection">
                            <rdf:Description rdf:about="http://www.w3.org/2004/02/skos/core#Concept"/>
                            <owl:Restriction>
                                <owl:onProperty rdf:resource="http://www.w3.org/2004/02/skos/core#inScheme"/>
                                <owl:hasValue rdf:resource="https://w3id.org/transmodel/kos/facilities/FacilityType"/>
                            </owl:Restriction>
                        </owl:intersectionOf>
                    </owl:Class>
                </owl:onClass>
            </owl:Restriction>
        </rdfs:subClassOf>
        <rdfs:subClassOf>
            <owl:Restriction>
                <owl:onProperty rdf:resource="https://w3id.org/transmodel/facilities#toiletFacility"/>
                <owl:maxQualifiedCardinality rdf:datatype="http://www.w3.org/2001/XMLSchema#nonNegativeInteger">1</owl:maxQualifiedCardinality>
                <owl:onClass>
                    <owl:Class>
                        <owl:intersectionOf rdf:parseType="Collection">
                            <rdf:Description rdf:about="http://www.w3.org/2004/02/skos/core#Concept"/>
                            <owl:Restriction>
                                <owl:onProperty rdf:resource="http://www.w3.org/2004/02/skos/core#inScheme"/>
                                <owl:hasValue rdf:resource="https://w3id.org/transmodel/kos/facilities/FacilityType"/>
                            </owl:Restriction>
                        </owl:intersectionOf>
                    </owl:Class>
                </owl:onClass>
            </owl:Restriction>
        </rdfs:subClassOf>
        <rdfs:comment xml:lang="en">This is a subclass of Service Facility Set to refer to types of accommodations, according to the Facility Conceptual Model (figure 287, page 450) of TransModel</rdfs:comment>
        <rdfs:label xml:lang="en">Accommodation</rdfs:label>
    </owl:Class>
    


    <!-- https://w3id.org/transmodel/facilities#ActivationLink -->

    <owl:Class rdf:about="https://w3id.org/transmodel/facilities#ActivationLink">
        <rdfs:subClassOf rdf:resource="https://w3id.org/transmodel/facilities#THINGSTOREVIEW"/>
        <rdfs:comment xml:lang="en">A Link where a control process is acivated when a vehicle passes it.</rdfs:comment>
        <rdfs:label xml:lang="en">ActivationLink</rdfs:label>
    </owl:Class>
    


    <!-- https://w3id.org/transmodel/facilities#ActivationPoint -->

    <owl:Class rdf:about="https://w3id.org/transmodel/facilities#ActivationPoint">
        <rdfs:subClassOf rdf:resource="https://w3id.org/transmodel/journeys#Point"/>
        <rdfs:comment xml:lang="en">A Point where a control process is activated when a vehicle passes it. equipment may be needed for activation.</rdfs:comment>
        <rdfs:label xml:lang="en">ActivationPoint</rdfs:label>
    </owl:Class>
    


    <!-- https://w3id.org/transmodel/facilities#AssistanceForDissabledUsers -->

    <owl:Class rdf:about="https://w3id.org/transmodel/facilities#AssistanceForDissabledUsers">
        <rdfs:subClassOf rdf:resource="https://w3id.org/transmodel/facilities#AssistanceService"/>
        <rdfs:comment xml:lang="en">Assistance Services for dissabled users of the Public Transport Network</rdfs:comment>
        <rdfs:comment xml:lang="en">TODO: Check if this has to be maintained, as it is not present in the Equipment Overview Physical Model of Transmodel (figure 247)</rdfs:comment>
        <rdfs:label xml:lang="en">AssistanceForDissabledUsers</rdfs:label>
    </owl:Class>
    


    <!-- https://w3id.org/transmodel/facilities#AssistanceService -->

    <owl:Class rdf:about="https://w3id.org/transmodel/facilities#AssistanceService">
        <rdfs:subClassOf rdf:resource="https://w3id.org/transmodel/facilities#LocalService"/>
        <rdfs:comment xml:lang="en">Specialisation of LocalService for Assistance providing information like language, accessibility trained staff, etc.</rdfs:comment>
        <rdfs:label xml:lang="en">AssistanceService</rdfs:label>
    </owl:Class>
    


    <!-- https://w3id.org/transmodel/facilities#BabyChange -->

    <owl:Class rdf:about="https://w3id.org/transmodel/facilities#BabyChange">
        <rdfs:subClassOf rdf:resource="https://w3id.org/transmodel/facilities#SanitaryEquipment"/>
        <rdfs:comment xml:lang="en">TODO: Check if this has to be maintained, as it is not present in the Equipment Overview Physical Model of Transmodel (figure 247)</rdfs:comment>
    </owl:Class>
    


    <!-- https://w3id.org/transmodel/facilities#BookingOffice -->

    <owl:Class rdf:about="https://w3id.org/transmodel/facilities#BookingOffice">
        <rdfs:subClassOf rdf:resource="https://w3id.org/transmodel/facilities#CustomerService"/>
        <rdfs:comment xml:lang="en">A specialisation of Customer Services for booking services</rdfs:comment>
        <rdfs:comment xml:lang="en">TODO: Check if this has to be maintained, as it is not present in the Equipment Overview Physical Model of Transmodel (figure 247)</rdfs:comment>
        <rdfs:label xml:lang="en">BookingOffice</rdfs:label>
    </owl:Class>
    


    <!-- https://w3id.org/transmodel/facilities#CateringService -->

    <owl:Class rdf:about="https://w3id.org/transmodel/facilities#CateringService">
        <rdfs:subClassOf rdf:resource="https://w3id.org/transmodel/facilities#CommercialService"/>
        <rdfs:comment xml:lang="en">Specialisation of LocalService for CateringService</rdfs:comment>
        <rdfs:label xml:lang="en">CateringService</rdfs:label>
    </owl:Class>
    


    <!-- https://w3id.org/transmodel/facilities#CheckIn -->

    <owl:Class rdf:about="https://w3id.org/transmodel/facilities#CheckIn">
        <rdfs:subClassOf rdf:resource="https://w3id.org/transmodel/facilities#EquipmentPlace"/>
        <rdfs:comment xml:lang="en">One specialisation of SiteComponent for Check in services</rdfs:comment>
        <rdfs:comment xml:lang="en">TODO: Check whether this has to be maintained, as it does not seem to appear clearly in any of the conceptual or implementation models of Transmodel</rdfs:comment>
        <rdfs:label xml:lang="en">CheckIn</rdfs:label>
    </owl:Class>
    


    <!-- https://w3id.org/transmodel/facilities#CommercialService -->

    <owl:Class rdf:about="https://w3id.org/transmodel/facilities#CommercialService">
        <rdfs:subClassOf rdf:resource="https://w3id.org/transmodel/facilities#LocalService"/>
        <rdfs:comment xml:lang="en">CommercialService is the specialisation of services for commercial purposes</rdfs:comment>
        <rdfs:comment xml:lang="en">TODO: Check if this has to be maintained as a classification or only keep them in a flat list, as it is proposed in the Equipment Overview Physical Model of Transmodel (figure 247)</rdfs:comment>
        <rdfs:label xml:lang="en">CommercialService</rdfs:label>
    </owl:Class>
    


    <!-- https://w3id.org/transmodel/facilities#CommunicationService -->

    <owl:Class rdf:about="https://w3id.org/transmodel/facilities#CommunicationService">
        <rdfs:subClassOf rdf:resource="https://w3id.org/transmodel/facilities#CommercialService"/>
        <rdfs:comment xml:lang="en">Specialisation of LocalService dedicated to communication services</rdfs:comment>
        <rdfs:label xml:lang="en">CommunicationService</rdfs:label>
    </owl:Class>
    


    <!-- https://w3id.org/transmodel/facilities#ComplaintsService -->

    <owl:Class rdf:about="https://w3id.org/transmodel/facilities#ComplaintsService">
        <rdfs:subClassOf rdf:resource="https://w3id.org/transmodel/facilities#CustomerService"/>
        <rdfs:comment xml:lang="en">Specialisation of CustomerService for Complaints Services</rdfs:comment>
        <rdfs:label xml:lang="en">ComplaintsService</rdfs:label>
    </owl:Class>
    


    <!-- https://w3id.org/transmodel/facilities#Constraint -->

    <owl:Class rdf:about="https://w3id.org/transmodel/facilities#Constraint">
        <rdfs:subClassOf rdf:resource="https://w3id.org/transmodel/facilities#THINGSTOREVIEW"/>
        <rdfs:comment xml:lang="en">A constraint that can take place at a SiteComponent that may potentially incur a time penalty that should be allowed for when journey planning</rdfs:comment>
        <rdfs:comment xml:lang="en">Constraint</rdfs:comment>
    </owl:Class>
    


    <!-- https://w3id.org/transmodel/facilities#ConstraintDelay -->

    <owl:Class rdf:about="https://w3id.org/transmodel/facilities#ConstraintDelay">
        <rdfs:subClassOf rdf:resource="https://w3id.org/transmodel/facilities#Constraint"/>
        <rdfs:comment xml:lang="en">A time penalty associated with a Constraint</rdfs:comment>
        <rdfs:label xml:lang="en">ConstraintDelay</rdfs:label>
    </owl:Class>
    


    <!-- https://w3id.org/transmodel/facilities#ConstraintOfAccess -->

    <owl:Class rdf:about="https://w3id.org/transmodel/facilities#ConstraintOfAccess">
        <rdfs:subClassOf rdf:resource="https://w3id.org/transmodel/facilities#Constraint"/>
        <rdfs:comment xml:lang="en">Access feature for CheckConstraint</rdfs:comment>
        <rdfs:label xml:lang="en">ConstraintOfAccess</rdfs:label>
    </owl:Class>
    


    <!-- https://w3id.org/transmodel/facilities#ConstraintThroughput -->

    <owl:Class rdf:about="https://w3id.org/transmodel/facilities#ConstraintThroughput">
        <rdfs:subClassOf rdf:resource="https://w3id.org/transmodel/facilities#Constraint"/>
        <rdfs:comment xml:lang="en">ConstraintThroughput is the throughput of a Constraint: the number of passenger who can pass through it in a specified interval</rdfs:comment>
        <rdfs:label xml:lang="en">ConstraintThroughput</rdfs:label>
    </owl:Class>
    


    <!-- https://w3id.org/transmodel/facilities#CrossingEquipment -->

    <owl:Class rdf:about="https://w3id.org/transmodel/facilities#CrossingEquipment">
        <rdfs:subClassOf rdf:resource="https://w3id.org/transmodel/facilities#AccessEquipment"/>
        <rdfs:comment xml:lang="en">Specialisation of PlaceAccessEquipment for CrossingEquipment

- Zebra</rdfs:comment>
        <rdfs:label xml:lang="en">CrossingEquipment</rdfs:label>
    </owl:Class>
    


    <!-- https://w3id.org/transmodel/facilities#CrossingEquipmentLights -->

    <owl:Class rdf:about="https://w3id.org/transmodel/facilities#CrossingEquipmentLights">
        <rdfs:subClassOf rdf:resource="https://w3id.org/transmodel/facilities#CrossingEquipment"/>
        <rdfs:comment xml:lang="en">TODO: Check if this has to be maintained, as it is not present in the Equipment Overview Physical Model of Transmodel (figure 247)</rdfs:comment>
    </owl:Class>
    


    <!-- https://w3id.org/transmodel/facilities#CrossingEquipmentPedestrian -->

    <owl:Class rdf:about="https://w3id.org/transmodel/facilities#CrossingEquipmentPedestrian">
        <rdfs:subClassOf rdf:resource="https://w3id.org/transmodel/facilities#CrossingEquipment"/>
        <rdfs:comment xml:lang="en">TODO: Check if this has to be maintained, as it is not present in the Equipment Overview Physical Model of Transmodel (figure 247)</rdfs:comment>
    </owl:Class>
    


    <!-- https://w3id.org/transmodel/facilities#CrossingEquipmentTactileGuideStrip -->

    <owl:Class rdf:about="https://w3id.org/transmodel/facilities#CrossingEquipmentTactileGuideStrip">
        <rdfs:subClassOf rdf:resource="https://w3id.org/transmodel/facilities#CrossingEquipment"/>
        <rdfs:comment xml:lang="en">TODO: Check if this has to be maintained, as it is not present in the Equipment Overview Physical Model of Transmodel (figure 247)</rdfs:comment>
    </owl:Class>
    


    <!-- https://w3id.org/transmodel/facilities#CrossingEquipmentZebra -->

    <owl:Class rdf:about="https://w3id.org/transmodel/facilities#CrossingEquipmentZebra">
        <rdfs:subClassOf rdf:resource="https://w3id.org/transmodel/facilities#CrossingEquipment"/>
        <rdfs:comment xml:lang="en">TODO: Check if this has to be maintained, as it is not present in the Equipment Overview Physical Model of Transmodel (figure 247)</rdfs:comment>
    </owl:Class>
    


    <!-- https://w3id.org/transmodel/facilities#CustomerService -->

    <owl:Class rdf:about="https://w3id.org/transmodel/facilities#CustomerService">
        <rdfs:subClassOf rdf:resource="https://w3id.org/transmodel/facilities#LocalService"/>
        <rdfs:comment xml:lang="en">Generic specialisation of LocalService for CustomerServices (LostProperties, MeetingPoint, Complaiants, etc.)</rdfs:comment>
        <rdfs:label xml:lang="en">CustomerService</rdfs:label>
    </owl:Class>
    


    <!-- https://w3id.org/transmodel/facilities#CycleOperatingEquipment -->

    <owl:Class rdf:about="https://w3id.org/transmodel/facilities#CycleOperatingEquipment">
        <rdfs:subClassOf rdf:resource="https://w3id.org/transmodel/facilities#PlaceEquipment"/>
        <rdfs:comment xml:lang="en">A specialisation of PlaceEquipment describing cycle parking equipment</rdfs:comment>
        <rdfs:comment xml:lang="en">TODO: Check if this has to be maintained, as it is not present in the Equipment Overview Physical Model of Transmodel (figure 247)</rdfs:comment>
        <rdfs:label xml:lang="en">CycleStorageEquipment</rdfs:label>
    </owl:Class>
    


    <!-- https://w3id.org/transmodel/facilities#EmergencyService -->

    <owl:Class rdf:about="https://w3id.org/transmodel/facilities#EmergencyService">
        <rdfs:subClassOf rdf:resource="https://w3id.org/transmodel/facilities#LocalService"/>
        <rdfs:comment xml:lang="en">TODO: Check if this has to be maintained, as it is not present in the Equipment Overview Physical Model of Transmodel (figure 247)</rdfs:comment>
        <rdfs:label xml:lang="en">EmergencyService</rdfs:label>
    </owl:Class>
    


    <!-- https://w3id.org/transmodel/facilities#EncumbranceNeed -->

    <owl:Class rdf:about="https://w3id.org/transmodel/facilities#EncumbranceNeed">
        <rdfs:subClassOf rdf:resource="https://w3id.org/transmodel/facilities#UserNeed"/>
        <rdfs:comment xml:lang="en">A specific UserNeed, i.e. a requirement of a Passenger travelling with luggage, animal or any other object requiring special arrangements to access PublicTransport</rdfs:comment>
        <rdfs:label xml:lang="en">EncumbranceNeed</rdfs:label>
    </owl:Class>
    


    <!-- https://w3id.org/transmodel/facilities#Entrance -->

    <owl:Class rdf:about="https://w3id.org/transmodel/facilities#Entrance">
        <rdfs:comment xml:lang="en">A physical entrance or exit to/from a Site. May be a door, barrier, gate or other recognizable Point of Access.</rdfs:comment>
        <rdfs:label xml:lang="en">Entrance</rdfs:label>
    </owl:Class>
    


    <!-- https://w3id.org/transmodel/facilities#EntranceEquipment -->

    <owl:Class rdf:about="https://w3id.org/transmodel/facilities#EntranceEquipment">
        <rdfs:subClassOf rdf:resource="https://w3id.org/transmodel/facilities#AccessEquipment"/>
        <rdfs:comment xml:lang="en">Specialisation of PlaceAccessEquipment for Entrances (door, barrier, gate or other recognizable point of access)</rdfs:comment>
        <rdfs:label xml:lang="en">EntranceEquipment</rdfs:label>
    </owl:Class>
    


    <!-- https://w3id.org/transmodel/facilities#Equipment -->

    <owl:Class rdf:about="https://w3id.org/transmodel/facilities#Equipment">
        <rdfs:subClassOf>
            <owl:Restriction>
                <owl:onProperty rdf:resource="https://w3id.org/transmodel/facilities#equipmentType"/>
                <owl:allValuesFrom>
                    <owl:Class>
                        <owl:intersectionOf rdf:parseType="Collection">
                            <rdf:Description rdf:about="http://www.w3.org/2004/02/skos/core#Concept"/>
                            <owl:Restriction>
                                <owl:onProperty rdf:resource="http://www.w3.org/2004/02/skos/core#inScheme"/>
                                <owl:hasValue rdf:resource="https://w3id.org/transmodel/kos/facilities/EquipmentType"/>
                            </owl:Restriction>
                        </owl:intersectionOf>
                    </owl:Class>
                </owl:allValuesFrom>
            </owl:Restriction>
        </rdfs:subClassOf>
        <rdfs:subClassOf>
            <owl:Restriction>
                <owl:onProperty rdf:resource="https://w3id.org/transmodel/facilities#locatedIn"/>
                <owl:maxQualifiedCardinality rdf:datatype="http://www.w3.org/2001/XMLSchema#nonNegativeInteger">1</owl:maxQualifiedCardinality>
                <owl:onClass rdf:resource="https://w3id.org/transmodel/facilities#EquipmentPlace"/>
            </owl:Restriction>
        </rdfs:subClassOf>
        <rdfs:subClassOf>
            <owl:Restriction>
                <owl:onProperty rdf:resource="https://w3id.org/transmodel/facilities#outOfService"/>
                <owl:maxQualifiedCardinality rdf:datatype="http://www.w3.org/2001/XMLSchema#nonNegativeInteger">1</owl:maxQualifiedCardinality>
                <owl:onDataRange rdf:resource="http://www.w3.org/2001/XMLSchema#boolean"/>
            </owl:Restriction>
        </rdfs:subClassOf>
        <rdfs:comment xml:lang="en">An equipment that may be located on a Vehicle, Site, etc. There are many different types of equipment, each of which may have specific properties (hence a large classification of concepts is provided as subclasses of this class).

The two main specialisations are Local Service and Installed Equipment.

A Local Service is an intangible service that is provided at a site, such as selling tickets, porterage, etc.

An Installed Equipment is the fixed equipment that may be installed fixed on a site (Place Equipment - e.g., door, lift, gate, etc.) or a vehicle (Vehicle Equipment), or mixed (e.g., rubish bins, sanitary equipment or ticketing equipments).

These are further characterised as Place Equipment (equipment which may be located only on a SITE, such as a barrier, bench, lift) and Passenger Equipment (equipment which may be located on either a Vehicle or a Site, such as a display terminal, ticket validator or WC)</rdfs:comment>
        <rdfs:label xml:lang="en">Equipment</rdfs:label>
    </owl:Class>
    


    <!-- https://w3id.org/transmodel/facilities#EquipmentPlace -->

    <owl:Class rdf:about="https://w3id.org/transmodel/facilities#EquipmentPlace">
        <rdfs:subClassOf rdf:resource="https://w3id.org/transmodel/facilities#SiteComponent"/>
        <rdfs:subClassOf>
            <owl:Restriction>
                <owl:onProperty rdf:resource="https://w3id.org/transmodel/facilities#equippedWith"/>
                <owl:allValuesFrom rdf:resource="https://w3id.org/transmodel/facilities#Equipment"/>
            </owl:Restriction>
        </rdfs:subClassOf>
        <rdfs:subClassOf>
            <owl:Restriction>
                <owl:onProperty rdf:resource="https://w3id.org/transmodel/facilities#position"/>
                <owl:allValuesFrom rdf:resource="https://w3id.org/transmodel/facilities#EquipmentPosition"/>
            </owl:Restriction>
        </rdfs:subClassOf>
        <rdfs:comment>An Equipment Place is a Site Component containing Equipment</rdfs:comment>
        <rdfs:label>Equipment Place</rdfs:label>
    </owl:Class>
    


    <!-- https://w3id.org/transmodel/facilities#EquipmentPosition -->

    <owl:Class rdf:about="https://w3id.org/transmodel/facilities#EquipmentPosition">
        <rdfs:comment xml:lang="en">TODO: Add a geolocation property for the position (most probably it will be a GeoSPARQL property, or a relationship to geo:Point)</rdfs:comment>
        <rdfs:comment xml:lang="en">The position that an equipment has, which comes with geospatial information and a description</rdfs:comment>
        <rdfs:label xml:lang="en">Equipment Position</rdfs:label>
    </owl:Class>
    


    <!-- https://w3id.org/transmodel/facilities#EscalatorEquipment -->

    <owl:Class rdf:about="https://w3id.org/transmodel/facilities#EscalatorEquipment">
        <rdfs:subClassOf rdf:resource="https://w3id.org/transmodel/facilities#StairEquipment"/>
        <rdfs:comment xml:lang="en">Specialisation of StairEquipment for Escalator Equipment</rdfs:comment>
        <rdfs:label xml:lang="en">EscalatorEquipment</rdfs:label>
    </owl:Class>
    


    <!-- https://w3id.org/transmodel/facilities#Facility -->

    <owl:Class rdf:about="https://w3id.org/transmodel/facilities#Facility">
        <rdfs:subClassOf>
            <owl:Restriction>
                <owl:onProperty rdf:resource="https://w3id.org/transmodel/facilities#facilityType"/>
                <owl:allValuesFrom>
                    <owl:Class>
                        <owl:intersectionOf rdf:parseType="Collection">
                            <rdf:Description rdf:about="http://www.w3.org/2004/02/skos/core#Concept"/>
                            <owl:Restriction>
                                <owl:onProperty rdf:resource="http://www.w3.org/2004/02/skos/core#inScheme"/>
                                <owl:hasValue rdf:resource="https://w3id.org/transmodel/kos/facilities/FacilityType"/>
                            </owl:Restriction>
                        </owl:intersectionOf>
                    </owl:Class>
                </owl:allValuesFrom>
            </owl:Restriction>
        </rdfs:subClassOf>
        <rdfs:comment xml:lang="en">A named amenity available to the public at a Site or on a Service.

A Facility has a type that determines the type of facility that it refers to, available in the SKOS codelist https://w3id.org/transmodel/kos/facilities/facilityType (in Netex this is represented as a set of enumerations)

A Facility has no further properties than a name. An Equipment or LocalService is used to describe the further properties provided as part of a particular Facility</rdfs:comment>
        <rdfs:label xml:lang="en">Facility</rdfs:label>
    </owl:Class>
    


    <!-- https://w3id.org/transmodel/facilities#FacilitySet -->

    <owl:Class rdf:about="https://w3id.org/transmodel/facilities#FacilitySet">
        <rdfs:subClassOf>
            <owl:Restriction>
                <owl:onProperty rdf:resource="https://w3id.org/transmodel/facilities#comprisesEquipment"/>
                <owl:allValuesFrom rdf:resource="https://w3id.org/transmodel/facilities#Equipment"/>
            </owl:Restriction>
        </rdfs:subClassOf>
        <rdfs:subClassOf>
            <owl:Restriction>
                <owl:onProperty rdf:resource="https://w3id.org/transmodel/facilities#comprisesFacility"/>
                <owl:allValuesFrom rdf:resource="https://w3id.org/transmodel/facilities#Facility"/>
            </owl:Restriction>
        </rdfs:subClassOf>
        <rdfs:comment xml:lang="en">A facility set is an aggregation of facilities. In Netex this is represented as a set of enumerated facility values (names based on TPEG classifications, augmented with UIC etc.).
The terms used for relating a facility set to the facilities and equipment are CommonFacilityGroup and otherFacilities. We have preferred using comprisesFacility and comprisesEquipment to simplify the terminology that is being used.</rdfs:comment>
        <rdfs:comment xml:lang="en">TODO: Add a restriction in subclassof for :providedBy only org:Organization</rdfs:comment>
        <rdfs:comment xml:lang="en">TODO: Transmodel also identifies as a potential restriction the assignment of 0 to N validity conditions to the Facility Set, but this has not been yet modelled</rdfs:comment>
        <rdfs:label xml:lang="en">Facility Set</rdfs:label>
    </owl:Class>
    


    <!-- https://w3id.org/transmodel/facilities#FlexibleStopPlace -->

    <owl:Class rdf:about="https://w3id.org/transmodel/facilities#FlexibleStopPlace">
        <rdfs:subClassOf rdf:resource="https://w3id.org/transmodel/facilities#StopPlace"/>
        <rdfs:comment xml:lang="en">A specialisation of the Stop Place describing a stop of a Flexible Service. It may be composed of Flexible Areas or Hail and Ride Areas identifying the catchment areas for flexible services (when they use areas or flexible quays). Some Flexible Places also use regular Stop Places for their stops. When assigned to a Scheduled Stop Point the corresponding Scheduled Stop Point is supposed to be a Zone (the centroid point of the Zone being the Scheduled Stop Point).</rdfs:comment>
        <rdfs:label xml:lang="en">Flexible Stop Place</rdfs:label>
    </owl:Class>
    


    <!-- https://w3id.org/transmodel/facilities#FreeWifi -->

    <owl:Class rdf:about="https://w3id.org/transmodel/facilities#FreeWifi">
        <rdfs:subClassOf rdf:resource="https://w3id.org/transmodel/facilities#CommunicationService"/>
        <rdfs:comment xml:lang="en">A private WiFi network that is available under certain characteristics</rdfs:comment>
        <rdfs:comment xml:lang="en">TODO: Check if this has to be maintained, as it is not present in the Equipment Overview Physical Model of Transmodel (figure 247)</rdfs:comment>
        <rdfs:label xml:lang="en">FreeWifi</rdfs:label>
    </owl:Class>
    


    <!-- https://w3id.org/transmodel/facilities#Garage -->

    <owl:Class rdf:about="https://w3id.org/transmodel/facilities#Garage">
        <rdfs:subClassOf rdf:resource="https://w3id.org/transmodel/facilities#PlaceEquipment"/>
        <rdfs:comment xml:lang="en">A Facility of PlaceEquipment used for parking and maintaining
	vehicles. Parking Point in a Garage are called GaragePoint.</rdfs:comment>
        <rdfs:comment xml:lang="en">TODO: Check if this has to be maintained, as it is not present in the Equipment Overview Physical Model of Transmodel (figure 247)</rdfs:comment>
        <rdfs:label xml:lang="en">Garage</rdfs:label>
    </owl:Class>
    


    <!-- https://w3id.org/transmodel/facilities#HeadingSign -->

    <owl:Class rdf:about="https://w3id.org/transmodel/facilities#HeadingSign">
        <rdfs:subClassOf rdf:resource="https://w3id.org/transmodel/facilities#SignEquipment"/>
        <rdfs:comment xml:lang="en">Specialisation of SignEquipment for headings providing information like direction name, line name, etc.</rdfs:comment>
        <rdfs:label xml:lang="en">HeadingSign</rdfs:label>
    </owl:Class>
    


    <!-- https://w3id.org/transmodel/facilities#HiringService -->

    <owl:Class rdf:about="https://w3id.org/transmodel/facilities#HiringService">
        <rdfs:subClassOf rdf:resource="https://w3id.org/transmodel/facilities#CommercialService"/>
        <rdfs:comment xml:lang="en">HiringService is the specialisation of CommercialService for hiring services</rdfs:comment>
        <rdfs:label xml:lang="en">HiringService</rdfs:label>
    </owl:Class>
    


    <!-- https://w3id.org/transmodel/facilities#Immigration -->

    <owl:Class rdf:about="https://w3id.org/transmodel/facilities#Immigration">
        <rdfs:subClassOf rdf:resource="https://w3id.org/transmodel/facilities#EquipmentPlace"/>
        <rdfs:comment xml:lang="en">One specialisation of SiteComponent for Migration affaires</rdfs:comment>
        <rdfs:comment xml:lang="en">TODO: Check whether this has to be maintained, as it does not seem to appear clearly in any of the conceptual or implementation models of Transmodel</rdfs:comment>
        <rdfs:label xml:lang="en">Immigration</rdfs:label>
    </owl:Class>
    


    <!-- https://w3id.org/transmodel/facilities#InformationBooklet -->

    <owl:Class rdf:about="https://w3id.org/transmodel/facilities#InformationBooklet">
        <rdfs:subClassOf rdf:resource="https://w3id.org/transmodel/facilities#PassengerInformationPrintedMaterial"/>
        <rdfs:comment xml:lang="en">Information Booklet is public transport piece of Equipment dedicated to inform</rdfs:comment>
        <rdfs:comment xml:lang="en">TODO: Check if this has to be maintained, as it is not present in the Equipment Overview Physical Model of Transmodel (figure 247)</rdfs:comment>
        <rdfs:label xml:lang="en">InformationBooklet</rdfs:label>
    </owl:Class>
    


    <!-- https://w3id.org/transmodel/facilities#InformationLeaflet -->

    <owl:Class rdf:about="https://w3id.org/transmodel/facilities#InformationLeaflet">
        <rdfs:subClassOf rdf:resource="https://w3id.org/transmodel/facilities#PassengerInformationPrintedMaterial"/>
        <rdfs:comment xml:lang="en">A public transport information piece of Equipment</rdfs:comment>
        <rdfs:comment xml:lang="en">TODO: Check if this has to be maintained, as it is not present in the Equipment Overview Physical Model of Transmodel (figure 247)</rdfs:comment>
        <rdfs:label xml:lang="en">InformationLeaflet</rdfs:label>
    </owl:Class>
    


    <!-- https://w3id.org/transmodel/facilities#InstalledEquipment -->

    <owl:Class rdf:about="https://w3id.org/transmodel/facilities#InstalledEquipment">
        <rdfs:subClassOf rdf:resource="https://w3id.org/transmodel/facilities#Equipment"/>
        <rdfs:comment xml:lang="en">An Installed Equipment is a fixed equipment that may be installed on a site (such as a door, lift, gate, etc.) or a vehicle. Its exact location may be specified by an Equipment Place. 
Physical equipments installed either fixed (PlaceEquipment), on-board (VehicleEquipment) or mixed (some equipments as rubish, sanitary or ticketing).</rdfs:comment>
        <rdfs:label xml:lang="en">Installed Equipment</rdfs:label>
    </owl:Class>
    


    <!-- https://w3id.org/transmodel/facilities#JourneyPattern -->

    <owl:Class rdf:about="https://w3id.org/transmodel/facilities#JourneyPattern">
        <rdfs:subClassOf rdf:resource="https://w3id.org/transmodel/facilities#THINGSTOREVIEW"/>
        <rdfs:label xml:lang="en">JourneyPattern</rdfs:label>
    </owl:Class>
    


    <!-- https://w3id.org/transmodel/facilities#LeftLuggageService -->

    <owl:Class rdf:about="https://w3id.org/transmodel/facilities#LeftLuggageService">
        <rdfs:subClassOf rdf:resource="https://w3id.org/transmodel/facilities#LuggageService"/>
        <rdfs:comment xml:lang="en">LeftLuggageService is the implementation of LuggageService for LeftLuggageService</rdfs:comment>
        <rdfs:label xml:lang="en">LeftLuggageService</rdfs:label>
    </owl:Class>
    


    <!-- https://w3id.org/transmodel/facilities#LiftEquipment -->

    <owl:Class rdf:about="https://w3id.org/transmodel/facilities#LiftEquipment">
        <rdfs:subClassOf rdf:resource="https://w3id.org/transmodel/facilities#AccessEquipment"/>
        <rdfs:comment xml:lang="en">Specialisation of PlaceAccessEquipment dedicated to PlaceAccessLift</rdfs:comment>
        <rdfs:label xml:lang="en">PlaceAccessLift</rdfs:label>
    </owl:Class>
    


    <!-- https://w3id.org/transmodel/facilities#LocalService -->

    <owl:Class rdf:about="https://w3id.org/transmodel/facilities#LocalService">
        <rdfs:subClassOf rdf:resource="https://w3id.org/transmodel/facilities#Equipment"/>
        <rdfs:comment xml:lang="en">A Service (LocalService such as LeftLuggage, TicketingService) is considered as immaterial Equipment as well.

A named Service relating to the use of the Site or transport Services at a particular location, for example Porterage, AssistanceForDissabledUsers, BookingOffices, etc. The Service may have a validityCondition associated with it.</rdfs:comment>
        <rdfs:label xml:lang="en">Service</rdfs:label>
    </owl:Class>
    


    <!-- https://w3id.org/transmodel/facilities#LostPropertieService -->

    <owl:Class rdf:about="https://w3id.org/transmodel/facilities#LostPropertieService">
        <rdfs:subClassOf rdf:resource="https://w3id.org/transmodel/facilities#CustomerService"/>
        <rdfs:comment xml:lang="en">Specialisation of CustomerService for LostProperties</rdfs:comment>
        <rdfs:label xml:lang="en">LostProperties</rdfs:label>
    </owl:Class>
    


    <!-- https://w3id.org/transmodel/facilities#LowFloor -->

    <owl:Class rdf:about="https://w3id.org/transmodel/facilities#LowFloor">
        <rdfs:subClassOf rdf:resource="https://w3id.org/transmodel/facilities#VehicleAccessEquipment"/>
        <rdfs:comment xml:lang="en">Specialisation of VehicleAccessEquipment dedicated to LowFloor</rdfs:comment>
        <rdfs:comment xml:lang="en">TODO: Check if this has to be maintained, as it is not present in the Equipment Overview Physical Model of Transmodel (figure 247)</rdfs:comment>
        <rdfs:label xml:lang="en">LowFloor</rdfs:label>
    </owl:Class>
    


    <!-- https://w3id.org/transmodel/facilities#LuggageLockerEquipment -->

    <owl:Class rdf:about="https://w3id.org/transmodel/facilities#LuggageLockerEquipment">
        <rdfs:subClassOf rdf:resource="https://w3id.org/transmodel/facilities#SiteEquipment"/>
        <rdfs:comment xml:lang="en">Specialisation of LuggageLockerEquipment for StopPlaceEquipment</rdfs:comment>
        <rdfs:label xml:lang="en">LuggageLockerEquipment</rdfs:label>
    </owl:Class>
    


    <!-- https://w3id.org/transmodel/facilities#LuggageService -->

    <owl:Class rdf:about="https://w3id.org/transmodel/facilities#LuggageService">
        <rdfs:subClassOf rdf:resource="https://w3id.org/transmodel/facilities#CustomerService"/>
        <rdfs:comment xml:lang="en">Specialisation of CustomerServices for LuggageServices.

Provides facilities as LuggageTrolley, FreeToUse, etc.</rdfs:comment>
        <rdfs:comment xml:lang="en">TODO: Check if this has to be maintained or moved to LocalService, as it is  present elsehwere in the Equipment Overview Physical Model of Transmodel (figure 247)</rdfs:comment>
        <rdfs:label xml:lang="en">LuggageService</rdfs:label>
    </owl:Class>
    


    <!-- https://w3id.org/transmodel/facilities#LuggageTrolleyService -->

    <owl:Class rdf:about="https://w3id.org/transmodel/facilities#LuggageTrolleyService">
        <rdfs:subClassOf rdf:resource="https://w3id.org/transmodel/facilities#LuggageService"/>
        <rdfs:comment xml:lang="en">TODO: Check if this has to be maintained, as it is not present in the Equipment Overview Physical Model of Transmodel (figure 247)</rdfs:comment>
        <rdfs:label xml:lang="en">LuggageTrolley</rdfs:label>
        <rdfs:label xml:lang="en">Specialisation of LuggageServices for LuggageTrolleyServices</rdfs:label>
    </owl:Class>
    


    <!-- https://w3id.org/transmodel/facilities#MeetingPointService -->

    <owl:Class rdf:about="https://w3id.org/transmodel/facilities#MeetingPointService">
        <rdfs:subClassOf rdf:resource="https://w3id.org/transmodel/facilities#CustomerService"/>
        <rdfs:comment xml:lang="en">Specialisation of CustomerService for meeting points (provides characteristics like description, labels...)</rdfs:comment>
        <rdfs:label xml:lang="en">MeetingPointService</rdfs:label>
    </owl:Class>
    


    <!-- https://w3id.org/transmodel/facilities#MoneyService -->

    <owl:Class rdf:about="https://w3id.org/transmodel/facilities#MoneyService">
        <rdfs:subClassOf rdf:resource="https://w3id.org/transmodel/facilities#CommercialService"/>
        <rdfs:comment xml:lang="en">MoneyService is the specialisation of Commercial services for money services. Provides information about money services.</rdfs:comment>
        <rdfs:label xml:lang="en">MoneyService</rdfs:label>
    </owl:Class>
    


    <!-- https://w3id.org/transmodel/facilities#Notice -->

    <owl:Class rdf:about="https://w3id.org/transmodel/facilities#Notice">
        <rdfs:subClassOf rdf:resource="https://w3id.org/transmodel/facilities#THINGSTOREVIEW"/>
        <rdfs:comment xml:lang="en">A text for informational purposes on exceptions in a Line, a Journey Pattern, etc. The information may be usable for Passenger or driver information</rdfs:comment>
        <rdfs:label xml:lang="en">Notice</rdfs:label>
    </owl:Class>
    


    <!-- https://w3id.org/transmodel/facilities#OnboardStay -->

    <owl:Class rdf:about="https://w3id.org/transmodel/facilities#OnboardStay">
        <rdfs:subClassOf rdf:resource="https://w3id.org/transmodel/facilities#Facility"/>
        <rdfs:subClassOf>
            <owl:Restriction>
                <owl:onProperty rdf:resource="https://w3id.org/transmodel/facilities#boardingPermission"/>
                <owl:maxQualifiedCardinality rdf:datatype="http://www.w3.org/2001/XMLSchema#nonNegativeInteger">1</owl:maxQualifiedCardinality>
                <owl:onClass>
                    <owl:Class>
                        <owl:intersectionOf rdf:parseType="Collection">
                            <rdf:Description rdf:about="http://www.w3.org/2004/02/skos/core#Concept"/>
                            <owl:Restriction>
                                <owl:onProperty rdf:resource="http://www.w3.org/2004/02/skos/core#inScheme"/>
                                <owl:hasValue rdf:resource="https://w3id.org/transmodel/kos/facilities/FacilityType"/>
                            </owl:Restriction>
                        </owl:intersectionOf>
                    </owl:Class>
                </owl:onClass>
            </owl:Restriction>
        </rdfs:subClassOf>
        <rdfs:subClassOf>
            <owl:Restriction>
                <owl:onProperty rdf:resource="https://w3id.org/transmodel/facilities#fareClass"/>
                <owl:maxQualifiedCardinality rdf:datatype="http://www.w3.org/2001/XMLSchema#nonNegativeInteger">1</owl:maxQualifiedCardinality>
                <owl:onClass>
                    <owl:Class>
                        <owl:intersectionOf rdf:parseType="Collection">
                            <rdf:Description rdf:about="http://www.w3.org/2004/02/skos/core#Concept"/>
                            <owl:Restriction>
                                <owl:onProperty rdf:resource="http://www.w3.org/2004/02/skos/core#inScheme"/>
                                <owl:hasValue rdf:resource="https://w3id.org/transmodel/kos/facilities/FacilityType"/>
                            </owl:Restriction>
                        </owl:intersectionOf>
                    </owl:Class>
                </owl:onClass>
            </owl:Restriction>
        </rdfs:subClassOf>
        <rdfs:subClassOf>
            <owl:Restriction>
                <owl:onProperty rdf:resource="https://w3id.org/transmodel/facilities#duration"/>
                <owl:maxQualifiedCardinality rdf:datatype="http://www.w3.org/2001/XMLSchema#nonNegativeInteger">1</owl:maxQualifiedCardinality>
                <owl:onDataRange rdf:resource="http://www.w3.org/2001/XMLSchema#duration"/>
            </owl:Restriction>
        </rdfs:subClassOf>
        <rdfs:comment xml:lang="en">This is a type of Service Facility Set, according to the Facility Conceptual Model (figure 287, page 450) of TransModel</rdfs:comment>
        <rdfs:label xml:lang="en">Onboard Stay</rdfs:label>
    </owl:Class>
    


    <!-- https://w3id.org/transmodel/facilities#OtherSign -->

    <owl:Class rdf:about="https://w3id.org/transmodel/facilities#OtherSign">
        <rdfs:subClassOf rdf:resource="https://w3id.org/transmodel/facilities#SignEquipment"/>
        <rdfs:comment xml:lang="en">Specialisation of SignEquipment which are not HeadingSign nor PlaceSign</rdfs:comment>
        <rdfs:label xml:lang="en">Other Sign</rdfs:label>
    </owl:Class>
    


    <!-- https://w3id.org/transmodel/facilities#Passenger -->

    <owl:Class rdf:about="https://w3id.org/transmodel/facilities#Passenger">
        <rdfs:subClassOf rdf:resource="https://w3id.org/transmodel/facilities#THINGSTOREVIEW"/>
        <rdfs:comment xml:lang="en">The Person who uses Public Transport Services</rdfs:comment>
        <rdfs:label xml:lang="en">Passenger</rdfs:label>
    </owl:Class>
    


    <!-- https://w3id.org/transmodel/facilities#PassengerArea -->

    <owl:Class rdf:about="https://w3id.org/transmodel/facilities#PassengerArea">
        <rdfs:subClassOf rdf:resource="https://w3id.org/transmodel/facilities#THINGSTOREVIEW"/>
        <rdfs:comment xml:lang="en">A Passenger Area within a StopPlace such as:
- Concourse
- Booking Hall
- Immigration Hall
- Security Area

Accessible by Passenger but without direct access to Vehicles</rdfs:comment>
        <rdfs:label xml:lang="en">PassengerArea</rdfs:label>
    </owl:Class>
    


    <!-- https://w3id.org/transmodel/facilities#PassengerEquipment -->

    <owl:Class rdf:about="https://w3id.org/transmodel/facilities#PassengerEquipment">
        <rdfs:subClassOf rdf:resource="https://w3id.org/transmodel/facilities#InstalledEquipment"/>
        <rdfs:subClassOf>
            <owl:Restriction>
                <owl:onProperty rdf:resource="https://w3id.org/transmodel/facilities#locatedIn"/>
                <owl:maxQualifiedCardinality rdf:datatype="http://www.w3.org/2001/XMLSchema#nonNegativeInteger">1</owl:maxQualifiedCardinality>
                <owl:onClass>
                    <owl:Class>
                        <owl:unionOf rdf:parseType="Collection">
                            <rdf:Description rdf:about="https://w3id.org/transmodel/facilities#EquipmentPlace"/>
                            <rdf:Description rdf:about="https://w3id.org/transmodel/facilities#Vehicle"/>
                        </owl:unionOf>
                    </owl:Class>
                </owl:onClass>
            </owl:Restriction>
        </rdfs:subClassOf>
        <rdfs:subClassOf>
            <owl:Restriction>
                <owl:onProperty rdf:resource="https://w3id.org/transmodel/facilities#fixed"/>
                <owl:maxQualifiedCardinality rdf:datatype="http://www.w3.org/2001/XMLSchema#nonNegativeInteger">1</owl:maxQualifiedCardinality>
                <owl:onDataRange rdf:resource="http://www.w3.org/2001/XMLSchema#boolean"/>
            </owl:Restriction>
        </rdfs:subClassOf>
        <rdfs:comment xml:lang="en">An item of equipment of a particular type actually available at a location within a Place (fixed) or a Vehicle (onboard)</rdfs:comment>
        <rdfs:label xml:lang="en">PassengerEquipment</rdfs:label>
    </owl:Class>
    


    <!-- https://w3id.org/transmodel/facilities#PassengerInformationEquipment -->

    <owl:Class rdf:about="https://w3id.org/transmodel/facilities#PassengerInformationEquipment">
        <rdfs:subClassOf rdf:resource="https://w3id.org/transmodel/facilities#PassengerEquipment"/>
        <rdfs:comment xml:lang="en">A public transport information piece of Equipment, as for instance terminals (on street, at information desks, telematic,...) or printed material (leaflets displayed at Stops, booklets, ...)</rdfs:comment>
        <rdfs:label xml:lang="en">PassengerInformationEquipment</rdfs:label>
    </owl:Class>
    


    <!-- https://w3id.org/transmodel/facilities#PassengerInformationPrintedMaterial -->

    <owl:Class rdf:about="https://w3id.org/transmodel/facilities#PassengerInformationPrintedMaterial">
        <rdfs:subClassOf rdf:resource="https://w3id.org/transmodel/facilities#PassengerInformationEquipment"/>
        <rdfs:comment xml:lang="en">A public transport information piece of Equipment which is printed material (leaflets displayed at Stops, booklets, ...)</rdfs:comment>
        <rdfs:comment xml:lang="en">TODO: Check if this has to be maintained, as it is not present in the Equipment Overview Physical Model of Transmodel (figure 247)</rdfs:comment>
        <rdfs:label xml:lang="en">PassengerInformationPrintedMaterial</rdfs:label>
    </owl:Class>
    


    <!-- https://w3id.org/transmodel/facilities#PassengerInformationTerminal -->

    <owl:Class rdf:about="https://w3id.org/transmodel/facilities#PassengerInformationTerminal">
        <rdfs:subClassOf rdf:resource="https://w3id.org/transmodel/facilities#PassengerInformationEquipment"/>
        <rdfs:comment xml:lang="en">A public transport information piece of equipment such as street stands, information desks or telematic services</rdfs:comment>
        <rdfs:comment xml:lang="en">TODO: Check if this has to be maintained, as it is not present in the Equipment Overview Physical Model of Transmodel (figure 247)</rdfs:comment>
        <rdfs:label xml:lang="en">PassengerInformationDesk</rdfs:label>
    </owl:Class>
    


    <!-- https://w3id.org/transmodel/facilities#PassengerSafetyEquipment -->

    <owl:Class rdf:about="https://w3id.org/transmodel/facilities#PassengerSafetyEquipment">
        <rdfs:subClassOf rdf:resource="https://w3id.org/transmodel/facilities#PassengerEquipment"/>
        <rdfs:label xml:lang="en">PassengerSafetyEquipment</rdfs:label>
    </owl:Class>
    


    <!-- https://w3id.org/transmodel/facilities#PlaceEquipment -->

    <owl:Class rdf:about="https://w3id.org/transmodel/facilities#PlaceEquipment">
        <rdfs:subClassOf rdf:resource="https://w3id.org/transmodel/facilities#InstalledEquipment"/>
        <rdfs:subClassOf>
            <owl:Class>
                <owl:intersectionOf rdf:parseType="Collection">
                    <owl:Restriction>
                        <owl:onProperty rdf:resource="https://w3id.org/transmodel/facilities#position"/>
                        <owl:someValuesFrom rdf:resource="https://w3id.org/transmodel/facilities#EquipmentPosition"/>
                    </owl:Restriction>
                    <owl:Restriction>
                        <owl:onProperty rdf:resource="https://w3id.org/transmodel/facilities#position"/>
                        <owl:maxQualifiedCardinality rdf:datatype="http://www.w3.org/2001/XMLSchema#nonNegativeInteger">1</owl:maxQualifiedCardinality>
                        <owl:onClass rdf:resource="https://w3id.org/transmodel/facilities#EquipmentPosition"/>
                    </owl:Restriction>
                </owl:intersectionOf>
            </owl:Class>
        </rdfs:subClassOf>
        <rdfs:subClassOf>
            <owl:Restriction>
                <owl:onProperty rdf:resource="https://w3id.org/transmodel/facilities#fixed"/>
                <owl:hasValue rdf:datatype="http://www.w3.org/2001/XMLSchema#boolean">true</owl:hasValue>
            </owl:Restriction>
        </rdfs:subClassOf>
        <rdfs:comment xml:lang="en">An item of Equipment of a particular type actually available at a location within a Place. It can only have one position</rdfs:comment>
        <rdfs:label xml:lang="en">PlaceEquipment</rdfs:label>
    </owl:Class>
    


    <!-- https://w3id.org/transmodel/facilities#PlaceLighting -->

    <owl:Class rdf:about="https://w3id.org/transmodel/facilities#PlaceLighting">
        <rdfs:subClassOf rdf:resource="https://w3id.org/transmodel/facilities#PlaceEquipment"/>
        <rdfs:comment xml:lang="en">Place Lighting</rdfs:comment>
    </owl:Class>
    


    <!-- https://w3id.org/transmodel/facilities#PlaceSign -->

    <owl:Class rdf:about="https://w3id.org/transmodel/facilities#PlaceSign">
        <rdfs:subClassOf rdf:resource="https://w3id.org/transmodel/facilities#SignEquipment"/>
        <rdfs:comment xml:lang="en">SignEquipment withe the name of a Place on it</rdfs:comment>
        <rdfs:label xml:lang="en">PlaceSign</rdfs:label>
    </owl:Class>
    


    <!-- https://w3id.org/transmodel/facilities#Porterage -->

    <owl:Class rdf:about="https://w3id.org/transmodel/facilities#Porterage">
        <rdfs:subClassOf rdf:resource="https://w3id.org/transmodel/facilities#LocalService"/>
        <rdfs:comment xml:lang="en">Porterage</rdfs:comment>
        <rdfs:comment xml:lang="en">PorterageService</rdfs:comment>
        <rdfs:comment xml:lang="en">TODO: Check if this has to be maintained, as it is not present in the Equipment Overview Physical Model of Transmodel (figure 247)</rdfs:comment>
    </owl:Class>
    


    <!-- https://w3id.org/transmodel/facilities#PostOfficeService -->

    <owl:Class rdf:about="https://w3id.org/transmodel/facilities#PostOfficeService">
        <rdfs:subClassOf rdf:resource="https://w3id.org/transmodel/facilities#CommunicationService"/>
        <rdfs:comment xml:lang="en">A PostOfficeService is the specialisation of CommunicationService for post mail services</rdfs:comment>
        <rdfs:comment xml:lang="en">TODO: Check if this has to be maintained, as it is not present in the Equipment Overview Physical Model of Transmodel (figure 247)</rdfs:comment>
        <rdfs:label xml:lang="en">PostOfficeService</rdfs:label>
    </owl:Class>
    


    <!-- https://w3id.org/transmodel/facilities#Quay -->

    <owl:Class rdf:about="https://w3id.org/transmodel/facilities#Quay">
        <rdfs:subClassOf>
            <owl:Restriction>
                <owl:onProperty rdf:resource="https://w3id.org/transmodel/commons#in"/>
                <owl:allValuesFrom rdf:resource="https://w3id.org/transmodel/facilities#StopPlace"/>
            </owl:Restriction>
        </rdfs:subClassOf>
        <rdfs:subClassOf>
            <owl:Restriction>
                <owl:onProperty rdf:resource="https://w3id.org/transmodel/facilities#comprises"/>
                <owl:allValuesFrom rdf:resource="https://w3id.org/transmodel/facilities#Quay"/>
            </owl:Restriction>
        </rdfs:subClassOf>
        <rdfs:comment xml:lang="en">A place such as platform, stance, or quayside where passengers have access to public transport vehicles, taxi, cars or other means of transportation. A Quay may serve one or more Vehicle Stopping Places and be associated with one or more Scheduled Stop Points. 

A Quay may contain other sub Quays</rdfs:comment>
        <rdfs:label xml:lang="en">Quay</rdfs:label>
    </owl:Class>
    


    <!-- https://w3id.org/transmodel/facilities#QueuingEquipment -->

    <owl:Class rdf:about="https://w3id.org/transmodel/facilities#QueuingEquipment">
        <rdfs:subClassOf rdf:resource="https://w3id.org/transmodel/facilities#AccessEquipment"/>
        <rdfs:label xml:lang="en">QueingEquipment</rdfs:label>
    </owl:Class>
    


    <!-- https://w3id.org/transmodel/facilities#Ramp -->

    <owl:Class rdf:about="https://w3id.org/transmodel/facilities#Ramp">
        <rdfs:subClassOf rdf:resource="https://w3id.org/transmodel/facilities#VehicleAccessEquipment"/>
        <rdfs:comment xml:lang="en">Specialisation of VehicleAccessEquipment dedicated to VehicleRamp</rdfs:comment>
        <rdfs:comment xml:lang="en">TODO: Check if this has to be maintained, as it is not present in the Equipment Overview Physical Model of Transmodel (figure 247)</rdfs:comment>
        <rdfs:label xml:lang="en">VehicleRamp</rdfs:label>
    </owl:Class>
    


    <!-- https://w3id.org/transmodel/facilities#RampEquipment -->

    <owl:Class rdf:about="https://w3id.org/transmodel/facilities#RampEquipment">
        <rdfs:subClassOf rdf:resource="https://w3id.org/transmodel/facilities#AccessEquipment"/>
        <rdfs:comment xml:lang="en">Specialisation of PlaceEquipment dedicated to access</rdfs:comment>
        <rdfs:label xml:lang="en">PlaceAccessRamp</rdfs:label>
    </owl:Class>
    


    <!-- https://w3id.org/transmodel/facilities#RetailService -->

    <owl:Class rdf:about="https://w3id.org/transmodel/facilities#RetailService">
        <rdfs:subClassOf rdf:resource="https://w3id.org/transmodel/facilities#CommercialService"/>
        <rdfs:comment xml:lang="en">Specialisation of LocalService dedicated to retail services</rdfs:comment>
        <rdfs:label xml:lang="en">RetailService</rdfs:label>
    </owl:Class>
    


    <!-- https://w3id.org/transmodel/facilities#RoughSurface -->

    <owl:Class rdf:about="https://w3id.org/transmodel/facilities#RoughSurface">
        <rdfs:subClassOf rdf:resource="https://w3id.org/transmodel/facilities#PlaceEquipment"/>
        <rdfs:label xml:lang="en">Rough Surface</rdfs:label>
    </owl:Class>
    


    <!-- https://w3id.org/transmodel/facilities#RubishDisposalEquipment -->

    <owl:Class rdf:about="https://w3id.org/transmodel/facilities#RubishDisposalEquipment">
        <rdfs:subClassOf rdf:resource="https://w3id.org/transmodel/facilities#PassengerEquipment"/>
        <rdfs:comment xml:lang="en">Specialisation of Passenger Equipment for Rubish Disposal</rdfs:comment>
        <rdfs:label xml:lang="en">RubishDisposal</rdfs:label>
    </owl:Class>
    


    <!-- https://w3id.org/transmodel/facilities#SanitaryEquipment -->

    <owl:Class rdf:about="https://w3id.org/transmodel/facilities#SanitaryEquipment">
        <rdfs:subClassOf rdf:resource="https://w3id.org/transmodel/facilities#PassengerEquipment"/>
        <rdfs:comment xml:lang="en">Specialisation of Passenger Equipment for Sanitary Equipment</rdfs:comment>
        <rdfs:label xml:lang="en">TypeOfSanitaryEquipment</rdfs:label>
    </owl:Class>
    


    <!-- https://w3id.org/transmodel/facilities#Screening -->

    <owl:Class rdf:about="https://w3id.org/transmodel/facilities#Screening">
        <rdfs:subClassOf rdf:resource="https://w3id.org/transmodel/facilities#EquipmentPlace"/>
        <rdfs:comment xml:lang="en">One specialisation of SiteComponent for Security Screening</rdfs:comment>
        <rdfs:comment xml:lang="en">TODO: Check whether this has to be maintained, as it does not seem to appear clearly in any of the conceptual or implementation models of Transmodel</rdfs:comment>
        <rdfs:label xml:lang="en">SecurityScreening</rdfs:label>
    </owl:Class>
    


    <!-- https://w3id.org/transmodel/facilities#SeatingEquipment -->

    <owl:Class rdf:about="https://w3id.org/transmodel/facilities#SeatingEquipment">
        <rdfs:subClassOf rdf:resource="https://w3id.org/transmodel/facilities#WaitingEquipment"/>
        <rdfs:label xml:lang="en">SeatingEquipment</rdfs:label>
    </owl:Class>
    


    <!-- https://w3id.org/transmodel/facilities#ServiceFacilitySet -->

    <owl:Class rdf:about="https://w3id.org/transmodel/facilities#ServiceFacilitySet">
        <rdfs:subClassOf rdf:resource="https://w3id.org/transmodel/facilities#FacilitySet"/>
        <rdfs:subClassOf>
            <owl:Restriction>
                <owl:onProperty rdf:resource="https://w3id.org/transmodel/facilities#presentAt"/>
                <owl:allValuesFrom rdf:resource="https://w3id.org/transmodel/facilities#VehicleType"/>
            </owl:Restriction>
        </rdfs:subClassOf>
        <rdfs:comment xml:lang="en">A service facility set contains a set of facilities available for a service journey or a journey part. The set may be availabe only for a specific vehicle type within the service (e.g., carriage equipped with low floor).
It can also include information about the accommodation on board, which can be related to the Accommodation or OnboardStay concepts, which are subclasses of Facility, via the comprisesFacility object property. These two concepts are further refined since they may have additional attributes beyond the indication of the corresponding SKOS concepts, as in the other cases.</rdfs:comment>
        <rdfs:comment xml:lang="en">TODO: Other class restrictions that may be added may include:
- for (inverse of made using), for Vehicle Journey and Coupled Journey (see figure 287, Facility conceptual Model)</rdfs:comment>
        <rdfs:label xml:lang="en">Service Facility Set</rdfs:label>
    </owl:Class>
    <owl:Axiom>
        <owl:annotatedSource rdf:resource="https://w3id.org/transmodel/facilities#ServiceFacilitySet"/>
        <owl:annotatedProperty rdf:resource="http://www.w3.org/2000/01/rdf-schema#subClassOf"/>
        <owl:annotatedTarget>
            <owl:Restriction>
                <owl:onProperty rdf:resource="https://w3id.org/transmodel/facilities#presentAt"/>
                <owl:allValuesFrom rdf:resource="https://w3id.org/transmodel/facilities#VehicleType"/>
            </owl:Restriction>
        </owl:annotatedTarget>
        <rdfs:comment>See figure 287, Facility conceptual Model</rdfs:comment>
    </owl:Axiom>
    


    <!-- https://w3id.org/transmodel/facilities#ShelterEquipment -->

    <owl:Class rdf:about="https://w3id.org/transmodel/facilities#ShelterEquipment">
        <rdfs:subClassOf rdf:resource="https://w3id.org/transmodel/facilities#WaitingEquipment"/>
        <rdfs:comment xml:lang="en">A building or other structure constructed at a Bus Stop</rdfs:comment>
        <rdfs:label xml:lang="en">Shelter</rdfs:label>
    </owl:Class>
    


    <!-- https://w3id.org/transmodel/facilities#Shower -->

    <owl:Class rdf:about="https://w3id.org/transmodel/facilities#Shower">
        <rdfs:subClassOf rdf:resource="https://w3id.org/transmodel/facilities#SanitaryEquipment"/>
        <rdfs:comment xml:lang="en">Specialisation of SanitaryEquipment for showers</rdfs:comment>
        <rdfs:comment xml:lang="en">TODO: Check if this has to be maintained, as it is not present in the Equipment Overview Physical Model of Transmodel (figure 247)</rdfs:comment>
        <rdfs:label xml:lang="en">Shower</rdfs:label>
    </owl:Class>
    


    <!-- https://w3id.org/transmodel/facilities#SignEquipment -->

    <owl:Class rdf:about="https://w3id.org/transmodel/facilities#SignEquipment">
        <rdfs:subClassOf rdf:resource="https://w3id.org/transmodel/facilities#PlaceEquipment"/>
        <rdfs:comment xml:lang="en">Specialisation of PlaceEquipment for Signs</rdfs:comment>
        <rdfs:label xml:lang="en">SignEquipment</rdfs:label>
    </owl:Class>
    


    <!-- https://w3id.org/transmodel/facilities#Site -->

    <owl:Class rdf:about="https://w3id.org/transmodel/facilities#Site">
        <rdfs:subClassOf>
            <owl:Restriction>
                <owl:onProperty rdf:resource="https://w3id.org/transmodel/facilities#concernedBy"/>
                <owl:allValuesFrom rdf:resource="https://w3id.org/transmodel/facilities#FacilitySet"/>
            </owl:Restriction>
        </rdfs:subClassOf>
        <rdfs:comment xml:lang="en">A well known Place to which Passengers may refer to indicate the origin or a destination of a Trip</rdfs:comment>
        <rdfs:label xml:lang="en">Site</rdfs:label>
    </owl:Class>
    


    <!-- https://w3id.org/transmodel/facilities#SiteComponent -->

    <owl:Class rdf:about="https://w3id.org/transmodel/facilities#SiteComponent">
        <rdfs:subClassOf rdf:resource="https://w3id.org/transmodel/facilities#SiteElement"/>
        <rdfs:comment xml:lang="en">An element of a Site describing a part of its structure. Site Components share common properties for data management, accessibility and other features</rdfs:comment>
        <rdfs:label xml:lang="en">Site Component</rdfs:label>
    </owl:Class>
    


    <!-- https://w3id.org/transmodel/facilities#SiteElement -->

    <owl:Class rdf:about="https://w3id.org/transmodel/facilities#SiteElement">
        <rdfs:subClassOf>
            <owl:Restriction>
                <owl:onProperty rdf:resource="https://w3id.org/transmodel/facilities#accessibilityAssessment"/>
                <owl:maxQualifiedCardinality rdf:datatype="http://www.w3.org/2001/XMLSchema#nonNegativeInteger">1</owl:maxQualifiedCardinality>
                <owl:onClass rdf:resource="https://w3id.org/transmodel/facilities#AccessibilityAssessment"/>
            </owl:Restriction>
        </rdfs:subClassOf>
        <rdfs:comment xml:lang="en">A place</rdfs:comment>
        <rdfs:comment xml:lang="en">TODO: Although the Transmodel conceptual model on Site Equipment specifies that a Site Element can only have one accessibility assessment, this may need to be relaxed to allow for more values to be included.</rdfs:comment>
        <rdfs:comment xml:lang="en">TODO: Check whether this should be related to a more general concept defining a place</rdfs:comment>
        <rdfs:label xml:lang="en">Site Element</rdfs:label>
    </owl:Class>
    


    <!-- https://w3id.org/transmodel/facilities#SiteEquipment -->

    <owl:Class rdf:about="https://w3id.org/transmodel/facilities#SiteEquipment">
        <rdfs:subClassOf rdf:resource="https://w3id.org/transmodel/facilities#PlaceEquipment"/>
        <rdfs:comment>Specialisation of PlaceEquipment for Site</rdfs:comment>
        <rdfs:label>SiteEquipment</rdfs:label>
    </owl:Class>
    


    <!-- https://w3id.org/transmodel/facilities#SiteFacilitySet -->

    <owl:Class rdf:about="https://w3id.org/transmodel/facilities#SiteFacilitySet">
        <rdfs:subClassOf rdf:resource="https://w3id.org/transmodel/facilities#FacilitySet"/>
        <rdfs:subClassOf>
            <owl:Restriction>
                <owl:onProperty rdf:resource="https://w3id.org/transmodel/facilities#availableAt"/>
                <owl:allValuesFrom rdf:resource="https://w3id.org/transmodel/facilities#Site"/>
            </owl:Restriction>
        </rdfs:subClassOf>
        <rdfs:comment xml:lang="en">A site facility set contains a set of facilities available at a site</rdfs:comment>
        <rdfs:label xml:lang="en">Site Facility Set</rdfs:label>
    </owl:Class>
    


    <!-- https://w3id.org/transmodel/facilities#StairCaseEquipment -->

    <owl:Class rdf:about="https://w3id.org/transmodel/facilities#StairCaseEquipment">
        <rdfs:subClassOf rdf:resource="https://w3id.org/transmodel/facilities#StairEquipment"/>
        <rdfs:comment xml:lang="en">Specialisation of PlaceAccessStair for StairCaseEquipment</rdfs:comment>
        <rdfs:label xml:lang="en">StairCaseEquipment</rdfs:label>
    </owl:Class>
    


    <!-- https://w3id.org/transmodel/facilities#StairEquipment -->

    <owl:Class rdf:about="https://w3id.org/transmodel/facilities#StairEquipment">
        <rdfs:subClassOf rdf:resource="https://w3id.org/transmodel/facilities#AccessEquipment"/>
        <rdfs:comment xml:lang="en">Specialisation of PlaceAccessEquipment dedicated to PlaceAccessStair (stair, escalator, staircase, etc.)</rdfs:comment>
        <rdfs:label xml:lang="en">PlaceAccessStair</rdfs:label>
    </owl:Class>
    


    <!-- https://w3id.org/transmodel/facilities#StatusOfEquipment -->

    <owl:Class rdf:about="https://w3id.org/transmodel/facilities#StatusOfEquipment">
        <rdfs:subClassOf rdf:resource="https://w3id.org/transmodel/facilities#THINGSTOREVIEW"/>
        <rdfs:label xml:lang="en">StatusOfEquipment</rdfs:label>
    </owl:Class>
    


    <!-- https://w3id.org/transmodel/facilities#StopPlace -->

    <owl:Class rdf:about="https://w3id.org/transmodel/facilities#StopPlace">
        <rdfs:subClassOf rdf:resource="https://w3id.org/transmodel/facilities#Site"/>
        <rdfs:subClassOf>
            <owl:Restriction>
                <owl:onProperty rdf:resource="https://w3id.org/transmodel/facilities#accessedBy"/>
                <owl:allValuesFrom rdf:resource="https://w3id.org/transmodel/facilities#StopPlaceEntrance"/>
            </owl:Restriction>
        </rdfs:subClassOf>
        <rdfs:subClassOf>
            <owl:Restriction>
                <owl:onProperty rdf:resource="https://w3id.org/transmodel/facilities#containing"/>
                <owl:allValuesFrom rdf:resource="https://w3id.org/transmodel/facilities#Quay"/>
            </owl:Restriction>
        </rdfs:subClassOf>
        <rdfs:subClassOf>
            <owl:Restriction>
                <owl:onProperty rdf:resource="https://w3id.org/transmodel/commons#borderCrossing"/>
                <owl:allValuesFrom rdf:resource="http://www.w3.org/2001/XMLSchema#boolean"/>
            </owl:Restriction>
        </rdfs:subClassOf>
        <rdfs:comment xml:lang="en">A place comprising one or more locations where Vehicles may stop and where passengers may board or leave Vehicles or prepare their Trip. A Stop Place will usually have one or more well-known names.</rdfs:comment>
        <rdfs:comment xml:lang="en">TODO: Add Stop Place Components to the Stop Place, if considered useful.</rdfs:comment>
        <rdfs:comment xml:lang="en">TODO: Add Stop Place Type as a SKOS Concept Scheme, and connect it to such concept scheme via an object property</rdfs:comment>
        <rdfs:comment xml:lang="en">TODO: If considered relevant, add connections from this class to the classes Point of Interest (this stop place services such Point of Interest) and to the class StopPlaceVehicleEntrance (this stop place is entered through an entrance - typical in an interchange area).</rdfs:comment>
        <rdfs:label xml:lang="en">Stop Place</rdfs:label>
    </owl:Class>
    


    <!-- https://w3id.org/transmodel/facilities#StopPlaceComponent -->

    <owl:Class rdf:about="https://w3id.org/transmodel/facilities#StopPlaceComponent">
        <rdfs:subClassOf rdf:resource="https://w3id.org/transmodel/facilities#THINGSTOREVIEW"/>
        <rdfs:comment xml:lang="en">An element of a StopPlace describing part of its structure. StopPlaceComponent share common properties for data management, accessibility and other features</rdfs:comment>
        <rdfs:label xml:lang="en">StopPlaceComponent</rdfs:label>
    </owl:Class>
    


    <!-- https://w3id.org/transmodel/facilities#StopPlaceEntrance -->

    <owl:Class rdf:about="https://w3id.org/transmodel/facilities#StopPlaceEntrance">
        <rdfs:subClassOf rdf:resource="https://w3id.org/transmodel/facilities#Entrance"/>
        <rdfs:comment xml:lang="en">A physical Entrance or Exit to/from a Stop Place for a Passenger. May be a door, barrier, gate or other recognizable point of access.</rdfs:comment>
        <rdfs:label xml:lang="en">Stop Place Entrance</rdfs:label>
    </owl:Class>
    


    <!-- https://w3id.org/transmodel/facilities#StopPlaceSpace -->

    <owl:Class rdf:about="https://w3id.org/transmodel/facilities#StopPlaceSpace">
        <rdfs:subClassOf rdf:resource="https://w3id.org/transmodel/facilities#THINGSTOREVIEW"/>
        <rdfs:comment xml:lang="en">A physical area within a StopPlace, for example, a Quay, BoardingPosition, AccessSpace or EquipmentPlace</rdfs:comment>
        <rdfs:label xml:lang="en">StopPlaceSpace</rdfs:label>
    </owl:Class>
    


    <!-- https://w3id.org/transmodel/facilities#Suitability -->

    <owl:Class rdf:about="https://w3id.org/transmodel/facilities#Suitability">
        <rdfs:subClassOf rdf:resource="https://w3id.org/transmodel/facilities#THINGSTOREVIEW"/>
        <rdfs:comment xml:lang="en">A statement of whether a particular UserNeed can be met. It can be used to state whether a Site can accessed by a Passenger with a particular UserNeed.</rdfs:comment>
        <rdfs:label xml:lang="en">Suitability</rdfs:label>
    </owl:Class>
    


    <!-- https://w3id.org/transmodel/facilities#THINGSTOREVIEW -->

    <owl:Class rdf:about="https://w3id.org/transmodel/facilities#THINGSTOREVIEW"/>
    


    <!-- https://w3id.org/transmodel/facilities#TicketControl -->

    <owl:Class rdf:about="https://w3id.org/transmodel/facilities#TicketControl">
        <rdfs:subClassOf rdf:resource="https://w3id.org/transmodel/facilities#EquipmentPlace"/>
        <rdfs:comment xml:lang="en">One specialisation of SiteComponent for Ticket control</rdfs:comment>
        <rdfs:comment xml:lang="en">TODO: Check whether this has to be maintained, as it does not seem to appear clearly in any of the conceptual or implementation models of Transmodel</rdfs:comment>
        <rdfs:label xml:lang="en">TicketControl</rdfs:label>
    </owl:Class>
    


    <!-- https://w3id.org/transmodel/facilities#TicketValidatorEquipment -->

    <owl:Class rdf:about="https://w3id.org/transmodel/facilities#TicketValidatorEquipment">
        <rdfs:subClassOf rdf:resource="https://w3id.org/transmodel/facilities#PassengerEquipment"/>
        <rdfs:comment xml:lang="en">Specialisation of Passenger Equipment for Ticket Validator Equipment</rdfs:comment>
        <rdfs:label xml:lang="en">TicketValidatorEquipment</rdfs:label>
    </owl:Class>
    


    <!-- https://w3id.org/transmodel/facilities#TicketingEquipment -->

    <owl:Class rdf:about="https://w3id.org/transmodel/facilities#TicketingEquipment">
        <rdfs:subClassOf rdf:resource="https://w3id.org/transmodel/facilities#PassengerEquipment"/>
        <rdfs:comment xml:lang="en">Specialisation of Passenter Equipment for Ticketing Equipment</rdfs:comment>
        <rdfs:label xml:lang="en">TicketingEquipment</rdfs:label>
    </owl:Class>
    


    <!-- https://w3id.org/transmodel/facilities#TicketingService -->

    <owl:Class rdf:about="https://w3id.org/transmodel/facilities#TicketingService">
        <rdfs:subClassOf rdf:resource="https://w3id.org/transmodel/facilities#LocalService"/>
        <rdfs:label xml:lang="en">TicketingService</rdfs:label>
    </owl:Class>
    


    <!-- https://w3id.org/transmodel/facilities#Toilet -->

    <owl:Class rdf:about="https://w3id.org/transmodel/facilities#Toilet">
        <rdfs:subClassOf rdf:resource="https://w3id.org/transmodel/facilities#SanitaryEquipment"/>
        <rdfs:comment xml:lang="en">TODO: Check if this has to be maintained, as it is not present in the Equipment Overview Physical Model of Transmodel (figure 247)</rdfs:comment>
        <rdfs:label xml:lang="en">Toilet</rdfs:label>
    </owl:Class>
    


    <!-- https://w3id.org/transmodel/facilities#TravelatorEquipment -->

    <owl:Class rdf:about="https://w3id.org/transmodel/facilities#TravelatorEquipment">
        <rdfs:subClassOf rdf:resource="https://w3id.org/transmodel/facilities#AccessEquipment"/>
    </owl:Class>
    


    <!-- https://w3id.org/transmodel/facilities#TrolleyStandEquipment -->

    <owl:Class rdf:about="https://w3id.org/transmodel/facilities#TrolleyStandEquipment">
        <rdfs:subClassOf rdf:resource="https://w3id.org/transmodel/facilities#SiteEquipment"/>
        <rdfs:comment xml:lang="en">Specialisation of StopPlaceEquipment for trolley stands</rdfs:comment>
        <rdfs:label xml:lang="en">TrolleyStandEquipment</rdfs:label>
    </owl:Class>
    


    <!-- https://w3id.org/transmodel/facilities#UserNeed -->

    <owl:Class rdf:about="https://w3id.org/transmodel/facilities#UserNeed">
        <rdfs:subClassOf rdf:resource="https://w3id.org/transmodel/facilities#THINGSTOREVIEW"/>
        <rdfs:comment xml:lang="en">A users&apos;s need for a particular Suitability</rdfs:comment>
        <rdfs:label xml:lang="en">UserNeed</rdfs:label>
    </owl:Class>
    


    <!-- https://w3id.org/transmodel/facilities#ValidityCondition -->

    <owl:Class rdf:about="https://w3id.org/transmodel/facilities#ValidityCondition">
        <rdfs:subClassOf rdf:resource="https://w3id.org/transmodel/facilities#THINGSTOREVIEW"/>
        <rdfs:comment xml:lang="en">Condition used in order to characterise a given Version of a VersionFrame. A ValidityCondition consists of a parameter (e.g. date, triggering event, etc.) and its type of application (e.g. for, from, until, etc.)</rdfs:comment>
        <rdfs:label xml:lang="en">ValidityCondition</rdfs:label>
    </owl:Class>
    


    <!-- https://w3id.org/transmodel/facilities#ValidityRuleParameter -->

    <owl:Class rdf:about="https://w3id.org/transmodel/facilities#ValidityRuleParameter">
        <rdfs:subClassOf rdf:resource="https://w3id.org/transmodel/facilities#ValidityCondition"/>
        <rdfs:comment xml:lang="en">A user defined ValidityCondition used by a rule for selecting versions. E.g. river level &gt; 1.5 m. and bad weather</rdfs:comment>
        <rdfs:label xml:lang="en">ValidityRuleParameter</rdfs:label>
    </owl:Class>
    


    <!-- https://w3id.org/transmodel/facilities#ValidityTrigger -->

    <owl:Class rdf:about="https://w3id.org/transmodel/facilities#ValidityTrigger">
        <rdfs:subClassOf rdf:resource="https://w3id.org/transmodel/facilities#THINGSTOREVIEW"/>
        <rdfs:comment xml:lang="en">External event defining a ValidityCondition. T. g. exceptional flow of a river, bad weather, road closure for works</rdfs:comment>
        <rdfs:label xml:lang="en">ValidityTrigger</rdfs:label>
    </owl:Class>
    


    <!-- https://w3id.org/transmodel/facilities#Vehicle -->

    <owl:Class rdf:about="https://w3id.org/transmodel/facilities#Vehicle">
        <rdfs:subClassOf rdf:resource="https://w3id.org/transmodel/facilities#THINGSTOREVIEW"/>
        <rdfs:comment xml:lang="en">A PublicTransportVehicle used for carrying Passenger</rdfs:comment>
        <rdfs:label xml:lang="en">Vehicle</rdfs:label>
    </owl:Class>
    


    <!-- https://w3id.org/transmodel/facilities#VehicleAccessEquipment -->

    <owl:Class rdf:about="https://w3id.org/transmodel/facilities#VehicleAccessEquipment">
        <rdfs:subClassOf rdf:resource="https://w3id.org/transmodel/facilities#VehicleEquipment"/>
        <rdfs:comment xml:lang="en">Specialisation of VehicleEquipment dedicated to access Vehicles providing information such as low floor, ramp, access area dimensions, etc.</rdfs:comment>
        <rdfs:label xml:lang="en">VehicleAccessEquipment</rdfs:label>
    </owl:Class>
    


    <!-- https://w3id.org/transmodel/facilities#VehicleChargingEquipment -->

    <owl:Class rdf:about="https://w3id.org/transmodel/facilities#VehicleChargingEquipment">
        <rdfs:subClassOf rdf:resource="https://w3id.org/transmodel/facilities#PlaceEquipment"/>
        <rdfs:comment xml:lang="en">Specialisation of PlaceEquipment for Vehicle charging</rdfs:comment>
        <rdfs:label xml:lang="en">VehicleChargingEquipment</rdfs:label>
    </owl:Class>
    


    <!-- https://w3id.org/transmodel/facilities#VehicleDisplayEquipment -->

    <owl:Class rdf:about="https://w3id.org/transmodel/facilities#VehicleDisplayEquipment">
        <rdfs:subClassOf rdf:resource="https://w3id.org/transmodel/facilities#PassengerInformationEquipment"/>
        <rdfs:comment xml:lang="en">TODO: Check if this has to be maintained, as it is not present in the Equipment Overview Physical Model of Transmodel (figure 247)</rdfs:comment>
        <rdfs:label xml:lang="en">PassengerInformationOnBoard</rdfs:label>
    </owl:Class>
    


    <!-- https://w3id.org/transmodel/facilities#VehicleEquipment -->

    <owl:Class rdf:about="https://w3id.org/transmodel/facilities#VehicleEquipment">
        <rdfs:subClassOf rdf:resource="https://w3id.org/transmodel/facilities#InstalledEquipment"/>
        <rdfs:subClassOf>
            <owl:Restriction>
                <owl:onProperty rdf:resource="https://w3id.org/transmodel/facilities#locatedIn"/>
                <owl:maxQualifiedCardinality rdf:datatype="http://www.w3.org/2001/XMLSchema#nonNegativeInteger">1</owl:maxQualifiedCardinality>
                <owl:onClass rdf:resource="https://w3id.org/transmodel/facilities#Vehicle"/>
            </owl:Restriction>
        </rdfs:subClassOf>
        <rdfs:comment xml:lang="en">A fixed equipment installed on a vehice. In Transmodel, this concept is called Actual Vehicle Equipment</rdfs:comment>
        <rdfs:comment xml:lang="en">TODO: check whether the range of the property locatedIn should go into the concept Vehicle from a different module of the ontology</rdfs:comment>
        <rdfs:label xml:lang="en">Vehicle Equipment</rdfs:label>
    </owl:Class>
    


    <!-- https://w3id.org/transmodel/facilities#VehicleMode -->

    <owl:Class rdf:about="https://w3id.org/transmodel/facilities#VehicleMode">
        <rdfs:subClassOf rdf:resource="https://w3id.org/transmodel/facilities#Vehicle"/>
        <rdfs:comment xml:lang="en">A classification of Public Transport Vehicles of the same Vehicle Type, e.g. according to Equipment specifications or model generation.</rdfs:comment>
        <rdfs:label xml:lang="en">VehicleModel</rdfs:label>
    </owl:Class>
    


    <!-- https://w3id.org/transmodel/facilities#VehicleStoppingPlace -->

    <owl:Class rdf:about="https://w3id.org/transmodel/facilities#VehicleStoppingPlace">
        <rdfs:subClassOf rdf:resource="https://w3id.org/transmodel/facilities#THINGSTOREVIEW"/>
        <rdfs:comment xml:lang="en">A place on the vehicle track where vehicles stop in order for passengers to board or alight from a vehicle.

A vehicle track is located on the respective infrastructure link for the mode (railway element of railway network, road element of road network, etc.).

A vehicle stopping place may be served by one or more quays.</rdfs:comment>
        <rdfs:label xml:lang="en">Vehicle Stopping Place</rdfs:label>
    </owl:Class>
    


    <!-- https://w3id.org/transmodel/facilities#VehicleType -->

    <owl:Class rdf:about="https://w3id.org/transmodel/facilities#VehicleType">
        <rdfs:subClassOf rdf:resource="https://w3id.org/transmodel/facilities#THINGSTOREVIEW"/>
        <rdfs:comment xml:lang="en">A classification of public transport vehicles according to the vehicle scheduling requirements in mode and capacity</rdfs:comment>
        <rdfs:label xml:lang="en">VehicleType</rdfs:label>
    </owl:Class>
    


    <!-- https://w3id.org/transmodel/facilities#WaitingEquipment -->

    <owl:Class rdf:about="https://w3id.org/transmodel/facilities#WaitingEquipment">
        <rdfs:subClassOf rdf:resource="https://w3id.org/transmodel/facilities#SiteEquipment"/>
        <rdfs:comment xml:lang="en">Specialisation of StopPlaceEquipment for WaitingEquipment (shelter, waiting room, etc.)</rdfs:comment>
        <rdfs:label xml:lang="en">WaitingEquipment</rdfs:label>
    </owl:Class>
    


    <!-- https://w3id.org/transmodel/facilities#WaitingRoomEquipment -->

    <owl:Class rdf:about="https://w3id.org/transmodel/facilities#WaitingRoomEquipment">
        <rdfs:subClassOf rdf:resource="https://w3id.org/transmodel/facilities#WaitingEquipment"/>
        <rdfs:subClassOf rdf:resource="https://w3id.org/transmodel/facilities#WaitingRoomEquipment"/>
        <rdfs:comment xml:lang="en">A Waiting Room</rdfs:comment>
        <rdfs:comment xml:lang="en">Specialisation of WaitingEquipment for WaitingRoom, classified by TypeOfWaitingRoom</rdfs:comment>
        <rdfs:label xml:lang="en">WaitingRoom</rdfs:label>
        <rdfs:label xml:lang="en">WaitingRoomEquipment</rdfs:label>
    </owl:Class>
    


    <!-- https://w3id.org/transmodel/facilities#WheelchairAccessToilet -->

    <owl:Class rdf:about="https://w3id.org/transmodel/facilities#WheelchairAccessToilet">
        <rdfs:subClassOf rdf:resource="https://w3id.org/transmodel/facilities#SanitaryEquipment"/>
        <rdfs:comment xml:lang="en">TODO: Check if this has to be maintained, as it is not present in the Equipment Overview Physical Model of Transmodel (figure 247)</rdfs:comment>
    </owl:Class>
    


    <!-- https://w3id.org/transmodel/facilities#WheelchairBabyChange -->

    <owl:Class rdf:about="https://w3id.org/transmodel/facilities#WheelchairBabyChange">
        <rdfs:subClassOf rdf:resource="https://w3id.org/transmodel/facilities#SanitaryEquipment"/>
        <rdfs:comment xml:lang="en">TODO: Check if this has to be maintained, as it is not present in the Equipment Overview Physical Model of Transmodel (figure 247)</rdfs:comment>
    </owl:Class>
    


    <!-- https://w3id.org/transmodel/facilities#WheelchairVehicleEquipment -->

    <owl:Class rdf:about="https://w3id.org/transmodel/facilities#WheelchairVehicleEquipment">
        <rdfs:subClassOf rdf:resource="https://w3id.org/transmodel/facilities#VehicleEquipment"/>
        <rdfs:comment xml:lang="en">Specialisation of Vehicle Equipment for wheel chair accessibility on board a Vehicle providing information suchs as the number of wheelchair areas and the access dimmensions</rdfs:comment>
        <rdfs:label xml:lang="en">WheelchairVehicleEquipment</rdfs:label>
    </owl:Class>
    


    <!-- https://w3id.org/transmodel/journeys#BeaconPoint -->

    <owl:Class rdf:about="https://w3id.org/transmodel/journeys#BeaconPoint">
        <rdfs:subClassOf rdf:resource="https://w3id.org/transmodel/journeys#Point"/>
        <rdfs:comment xml:lang="en">A Point where a beacon or similar device to support the automatic detection of vehicles passing by is located</rdfs:comment>
        <rdfs:label xml:lang="en">BeaconPoint</rdfs:label>
    </owl:Class>
    


    <!-- https://w3id.org/transmodel/journeys#Point -->

    <owl:Class rdf:about="https://w3id.org/transmodel/journeys#Point">
        <rdfs:subClassOf rdf:resource="https://w3id.org/transmodel/facilities#THINGSTOREVIEW"/>
        <rdfs:label xml:lang="en">Point</rdfs:label>
    </owl:Class>
    


    <!-- https://w3id.org/transmodel/journeys#Service -->

    <owl:Class rdf:about="https://w3id.org/transmodel/journeys#Service">
        <rdfs:subClassOf rdf:resource="https://w3id.org/transmodel/facilities#THINGSTOREVIEW"/>
        <rdfs:comment xml:lang="en">A ServiceJourney is a Passenger carrying VehicleJourney for one specified DayType. The pattern of working is in principle defined by a ServiceJourneyPattern.</rdfs:comment>
        <rdfs:comment>TODO: To remove once that we are sure that we are not breaking anything</rdfs:comment>
        <rdfs:label xml:lang="en">Service</rdfs:label>
    </owl:Class>
    


    <!-- 
    ///////////////////////////////////////////////////////////////////////////////////////
    //
    // Individuals
    //
    ///////////////////////////////////////////////////////////////////////////////////////
     -->

    


    <!-- https://w3id.org/transmodel/facilities#accessible -->

    <owl:NamedIndividual rdf:about="https://w3id.org/transmodel/facilities#accessible"/>
    


    <!-- https://w3id.org/transmodel/facilities#audioNavigator -->

    <owl:NamedIndividual rdf:about="https://w3id.org/transmodel/facilities#audioNavigator"/>
    


    <!-- https://w3id.org/transmodel/facilities#babychange -->

    <owl:NamedIndividual rdf:about="https://w3id.org/transmodel/facilities#babychange">
        <rdf:type rdf:resource="https://w3id.org/transmodel/facilities#SanitaryEquipment"/>
        <rdfs:label xml:lang="en">babyChange</rdfs:label>
    </owl:NamedIndividual>
    


    <!-- https://w3id.org/transmodel/facilities#baggageCheckin -->

    <owl:NamedIndividual rdf:about="https://w3id.org/transmodel/facilities#baggageCheckin"/>
    


    <!-- https://w3id.org/transmodel/facilities#barrier -->

    <owl:NamedIndividual rdf:about="https://w3id.org/transmodel/facilities#barrier">
        <rdfs:label xml:lang="en">barrierEntrance</rdfs:label>
    </owl:NamedIndividual>
    


    <!-- https://w3id.org/transmodel/facilities#beverageVendingMachine -->

    <owl:NamedIndividual rdf:about="https://w3id.org/transmodel/facilities#beverageVendingMachine"/>
    


    <!-- https://w3id.org/transmodel/facilities#bookingHall -->

    <owl:NamedIndividual rdf:about="https://w3id.org/transmodel/facilities#bookingHall">
        <rdf:type rdf:resource="https://w3id.org/transmodel/facilities#PassengerArea"/>
        <rdfs:label xml:lang="en">bookingHall</rdfs:label>
    </owl:NamedIndividual>
    


    <!-- https://w3id.org/transmodel/facilities#boundedOpenSpace -->

    <owl:NamedIndividual rdf:about="https://w3id.org/transmodel/facilities#boundedOpenSpace">
        <rdf:type rdf:resource="https://w3id.org/transmodel/facilities#PassengerArea"/>
    </owl:NamedIndividual>
    


    <!-- https://w3id.org/transmodel/facilities#buffet -->

    <owl:NamedIndividual rdf:about="https://w3id.org/transmodel/facilities#buffet"/>
    


    <!-- https://w3id.org/transmodel/facilities#bunk -->

    <owl:NamedIndividual rdf:about="https://w3id.org/transmodel/facilities#bunk"/>
    


    <!-- https://w3id.org/transmodel/facilities#cateringTrolleyService -->

    <owl:NamedIndividual rdf:about="https://w3id.org/transmodel/facilities#cateringTrolleyService"/>
    


    <!-- https://w3id.org/transmodel/facilities#compoundTrain -->

    <owl:NamedIndividual rdf:about="https://w3id.org/transmodel/facilities#compoundTrain">
        <rdf:type rdf:resource="https://w3id.org/transmodel/facilities#VehicleType"/>
        <rdfs:comment xml:lang="en">A VehicleType composed of a sequence of more than one vehicles of the type Train</rdfs:comment>
        <rdfs:label xml:lang="en">compoundTrain</rdfs:label>
    </owl:NamedIndividual>
    


    <!-- https://w3id.org/transmodel/facilities#concourse -->

    <owl:NamedIndividual rdf:about="https://w3id.org/transmodel/facilities#concourse">
        <rdf:type rdf:resource="https://w3id.org/transmodel/facilities#PassengerArea"/>
        <rdfs:label xml:lang="en">concourse</rdfs:label>
    </owl:NamedIndividual>
    


    <!-- https://w3id.org/transmodel/facilities#confinedSpace -->

    <owl:NamedIndividual rdf:about="https://w3id.org/transmodel/facilities#confinedSpace"/>
    


    <!-- https://w3id.org/transmodel/facilities#corridor -->

    <owl:NamedIndividual rdf:about="https://w3id.org/transmodel/facilities#corridor">
        <rdf:type rdf:resource="https://w3id.org/transmodel/facilities#PassengerArea"/>
    </owl:NamedIndividual>
    


    <!-- https://w3id.org/transmodel/facilities#couchette -->

    <owl:NamedIndividual rdf:about="https://w3id.org/transmodel/facilities#couchette"/>
    


    <!-- https://w3id.org/transmodel/facilities#crowding -->

    <owl:NamedIndividual rdf:about="https://w3id.org/transmodel/facilities#crowding"/>
    


    <!-- https://w3id.org/transmodel/facilities#cycleStorageEquipmentBars -->

    <owl:NamedIndividual rdf:about="https://w3id.org/transmodel/facilities#cycleStorageEquipmentBars"/>
    


    <!-- https://w3id.org/transmodel/facilities#cycleStorageEquipmentRacks -->

    <owl:NamedIndividual rdf:about="https://w3id.org/transmodel/facilities#cycleStorageEquipmentRacks"/>
    


    <!-- https://w3id.org/transmodel/facilities#cycleStorageEquipmentRailings -->

    <owl:NamedIndividual rdf:about="https://w3id.org/transmodel/facilities#cycleStorageEquipmentRailings"/>
    


    <!-- https://w3id.org/transmodel/facilities#directionName -->

    <owl:NamedIndividual rdf:about="https://w3id.org/transmodel/facilities#directionName">
        <rdf:type rdf:resource="https://w3id.org/transmodel/facilities#HeadingSign"/>
        <rdfs:label xml:lang="en">directionName</rdfs:label>
    </owl:NamedIndividual>
    


    <!-- https://w3id.org/transmodel/facilities#doubleDeck -->

    <owl:NamedIndividual rdf:about="https://w3id.org/transmodel/facilities#doubleDeck">
        <rdf:type rdf:resource="https://w3id.org/transmodel/facilities#VehicleType"/>
        <rdfs:label xml:lang="en">doubleDeck</rdfs:label>
    </owl:NamedIndividual>
    


    <!-- https://w3id.org/transmodel/facilities#emergencyServiceFirstAid -->

    <owl:NamedIndividual rdf:about="https://w3id.org/transmodel/facilities#emergencyServiceFirstAid"/>
    


    <!-- https://w3id.org/transmodel/facilities#emergencyServicePolice -->

    <owl:NamedIndividual rdf:about="https://w3id.org/transmodel/facilities#emergencyServicePolice"/>
    


    <!-- https://w3id.org/transmodel/facilities#emergencyServiceSOSPoint -->

    <owl:NamedIndividual rdf:about="https://w3id.org/transmodel/facilities#emergencyServiceSOSPoint"/>
    


    <!-- https://w3id.org/transmodel/facilities#emergencyServiceServiceCCTV -->

    <owl:NamedIndividual rdf:about="https://w3id.org/transmodel/facilities#emergencyServiceServiceCCTV"/>
    


    <!-- https://w3id.org/transmodel/facilities#entranceEquipmentBarrier -->

    <owl:NamedIndividual rdf:about="https://w3id.org/transmodel/facilities#entranceEquipmentBarrier"/>
    


    <!-- https://w3id.org/transmodel/facilities#entranceEquipmentDoor -->

    <owl:NamedIndividual rdf:about="https://w3id.org/transmodel/facilities#entranceEquipmentDoor">
        <rdfs:label xml:lang="en">entranceEquipmentDoor</rdfs:label>
    </owl:NamedIndividual>
    


    <!-- https://w3id.org/transmodel/facilities#entranceEquipmentRevolvingDoor -->

    <owl:NamedIndividual rdf:about="https://w3id.org/transmodel/facilities#entranceEquipmentRevolvingDoor">
        <rdfs:label xml:lang="en">entranceEquipmentRevolvingDoor</rdfs:label>
    </owl:NamedIndividual>
    


    <!-- https://w3id.org/transmodel/facilities#equipmentActivated -->

    <owl:NamedIndividual rdf:about="https://w3id.org/transmodel/facilities#equipmentActivated">
        <rdf:type rdf:resource="https://w3id.org/transmodel/facilities#StatusOfEquipment"/>
        <rdfs:label xml:lang="en">equipmentActivated</rdfs:label>
    </owl:NamedIndividual>
    


    <!-- https://w3id.org/transmodel/facilities#equipmentAtStopPoint -->

    <owl:NamedIndividual rdf:about="https://w3id.org/transmodel/facilities#equipmentAtStopPoint">
        <rdfs:label xml:lang="en">equipmentAtStopPoint</rdfs:label>
    </owl:NamedIndividual>
    


    <!-- https://w3id.org/transmodel/facilities#equipmentOnBoard -->

    <owl:NamedIndividual rdf:about="https://w3id.org/transmodel/facilities#equipmentOnBoard"/>
    


    <!-- https://w3id.org/transmodel/facilities#equipmentdesactvated -->

    <owl:NamedIndividual rdf:about="https://w3id.org/transmodel/facilities#equipmentdesactvated">
        <rdf:type rdf:resource="https://w3id.org/transmodel/facilities#StatusOfEquipment"/>
        <rdfs:label xml:lang="en">equipmentDesactivated</rdfs:label>
    </owl:NamedIndividual>
    


    <!-- https://w3id.org/transmodel/facilities#firstClass -->

    <owl:NamedIndividual rdf:about="https://w3id.org/transmodel/facilities#firstClass"/>
    


    <!-- https://w3id.org/transmodel/facilities#foodVendingMachine -->

    <owl:NamedIndividual rdf:about="https://w3id.org/transmodel/facilities#foodVendingMachine"/>
    


    <!-- https://w3id.org/transmodel/facilities#full -->

    <owl:NamedIndividual rdf:about="https://w3id.org/transmodel/facilities#full"/>
    


    <!-- https://w3id.org/transmodel/facilities#hall -->

    <owl:NamedIndividual rdf:about="https://w3id.org/transmodel/facilities#hall">
        <rdf:type rdf:resource="https://w3id.org/transmodel/facilities#PassengerArea"/>
    </owl:NamedIndividual>
    


    <!-- https://w3id.org/transmodel/facilities#handrailOneSide -->

    <owl:NamedIndividual rdf:about="https://w3id.org/transmodel/facilities#handrailOneSide"/>
    


    <!-- https://w3id.org/transmodel/facilities#handrailTwoSides -->

    <owl:NamedIndividual rdf:about="https://w3id.org/transmodel/facilities#handrailTwoSides"/>
    


    <!-- https://w3id.org/transmodel/facilities#immigrationHall -->

    <owl:NamedIndividual rdf:about="https://w3id.org/transmodel/facilities#immigrationHall">
        <rdf:type rdf:resource="https://w3id.org/transmodel/facilities#PassengerArea"/>
        <rdfs:label xml:lang="en">immigrationHall</rdfs:label>
    </owl:NamedIndividual>
    


    <!-- https://w3id.org/transmodel/facilities#incomingCustoms -->

    <owl:NamedIndividual rdf:about="https://w3id.org/transmodel/facilities#incomingCustoms"/>
    


    <!-- https://w3id.org/transmodel/facilities#informationDesk -->

    <owl:NamedIndividual rdf:about="https://w3id.org/transmodel/facilities#informationDesk">
        <rdfs:comment xml:lang="en">A public transport information piece of Equipment indoors</rdfs:comment>
        <rdfs:label xml:lang="en">InformationDesk</rdfs:label>
    </owl:NamedIndividual>
    


    <!-- https://w3id.org/transmodel/facilities#informationStand -->

    <owl:NamedIndividual rdf:about="https://w3id.org/transmodel/facilities#informationStand">
        <rdfs:comment xml:lang="en">A public transport information piece of Equipment outdoors</rdfs:comment>
        <rdfs:label xml:lang="en">informationStand</rdfs:label>
    </owl:NamedIndividual>
    


    <!-- https://w3id.org/transmodel/facilities#lift -->

    <owl:NamedIndividual rdf:about="https://w3id.org/transmodel/facilities#lift"/>
    


    <!-- https://w3id.org/transmodel/facilities#lineName -->

    <owl:NamedIndividual rdf:about="https://w3id.org/transmodel/facilities#lineName">
        <rdf:type rdf:resource="https://w3id.org/transmodel/facilities#HeadingSign"/>
        <rdfs:label xml:lang="en">lineName</rdfs:label>
    </owl:NamedIndividual>
    


    <!-- https://w3id.org/transmodel/facilities#lowFloor -->

    <owl:NamedIndividual rdf:about="https://w3id.org/transmodel/facilities#lowFloor">
        <rdfs:label xml:lang="en">lowFloor</rdfs:label>
    </owl:NamedIndividual>
    


    <!-- https://w3id.org/transmodel/facilities#narrowEntrance -->

    <owl:NamedIndividual rdf:about="https://w3id.org/transmodel/facilities#narrowEntrance">
        <rdfs:label xml:lang="en">narrowEntrance</rdfs:label>
    </owl:NamedIndividual>
    


    <!-- https://w3id.org/transmodel/facilities#noBeveragesAvailable -->

    <owl:NamedIndividual rdf:about="https://w3id.org/transmodel/facilities#noBeveragesAvailable">
        <rdfs:label xml:lang="en"></rdfs:label>
        <rdfs:label>beverages</rdfs:label>
    </owl:NamedIndividual>
    


    <!-- https://w3id.org/transmodel/facilities#noFoodAvailable -->

    <owl:NamedIndividual rdf:about="https://w3id.org/transmodel/facilities#noFoodAvailable">
        <rdfs:label xml:lang="en">food</rdfs:label>
    </owl:NamedIndividual>
    


    <!-- https://w3id.org/transmodel/facilities#noWaiting -->

    <owl:NamedIndividual rdf:about="https://w3id.org/transmodel/facilities#noWaiting"/>
    


    <!-- https://w3id.org/transmodel/facilities#nonAccessible -->

    <owl:NamedIndividual rdf:about="https://w3id.org/transmodel/facilities#nonAccessible"/>
    


    <!-- https://w3id.org/transmodel/facilities#outgoingCustoms -->

    <owl:NamedIndividual rdf:about="https://w3id.org/transmodel/facilities#outgoingCustoms"/>
    


    <!-- https://w3id.org/transmodel/facilities#placeAccessStairScalator -->

    <owl:NamedIndividual rdf:about="https://w3id.org/transmodel/facilities#placeAccessStairScalator">
        <rdfs:comment xml:lang="en">Specialisation of PlaceAccessStair Equipment dedicated to PlaceAccessStairEscalator</rdfs:comment>
        <rdfs:label xml:lang="en">placeAccessStairScalator</rdfs:label>
    </owl:NamedIndividual>
    


    <!-- https://w3id.org/transmodel/facilities#placeAccessStairStair -->

    <owl:NamedIndividual rdf:about="https://w3id.org/transmodel/facilities#placeAccessStairStair">
        <rdfs:comment xml:lang="en">Specialisation of PlaceAccessStair Equipment dedicated to PlaceAccessStairStair</rdfs:comment>
        <rdfs:label xml:lang="en">placeAccessStairStair</rdfs:label>
    </owl:NamedIndividual>
    


    <!-- https://w3id.org/transmodel/facilities#placeAccessStairStaircase -->

    <owl:NamedIndividual rdf:about="https://w3id.org/transmodel/facilities#placeAccessStairStaircase">
        <rdfs:comment xml:lang="en">Specialisation of PlaceAccessStair Equipment dedicated to PlaceAccessStairStaircase</rdfs:comment>
        <rdfs:label xml:lang="en">placeAccessStairStaircase</rdfs:label>
    </owl:NamedIndividual>
    


    <!-- https://w3id.org/transmodel/facilities#queue -->

    <owl:NamedIndividual rdf:about="https://w3id.org/transmodel/facilities#queue"/>
    


    <!-- https://w3id.org/transmodel/facilities#queueManagement -->

    <owl:NamedIndividual rdf:about="https://w3id.org/transmodel/facilities#queueManagement"/>
    


    <!-- https://w3id.org/transmodel/facilities#riverFlow -->

    <owl:NamedIndividual rdf:about="https://w3id.org/transmodel/facilities#riverFlow">
        <rdf:type rdf:resource="https://w3id.org/transmodel/facilities#ValidityTrigger"/>
        <rdfs:label xml:lang="en">riverFlow</rdfs:label>
    </owl:NamedIndividual>
    


    <!-- https://w3id.org/transmodel/facilities#roadClosure -->

    <owl:NamedIndividual rdf:about="https://w3id.org/transmodel/facilities#roadClosure">
        <rdf:type rdf:resource="https://w3id.org/transmodel/facilities#ValidityTrigger"/>
        <rdfs:label xml:lang="en">roadClosure</rdfs:label>
    </owl:NamedIndividual>
    


    <!-- https://w3id.org/transmodel/facilities#room -->

    <owl:NamedIndividual rdf:about="https://w3id.org/transmodel/facilities#room">
        <rdf:type rdf:resource="https://w3id.org/transmodel/facilities#PassengerArea"/>
    </owl:NamedIndividual>
    


    <!-- https://w3id.org/transmodel/facilities#secondClass -->

    <owl:NamedIndividual rdf:about="https://w3id.org/transmodel/facilities#secondClass"/>
    


    <!-- https://w3id.org/transmodel/facilities#securityArea -->

    <owl:NamedIndividual rdf:about="https://w3id.org/transmodel/facilities#securityArea">
        <rdf:type rdf:resource="https://w3id.org/transmodel/facilities#PassengerArea"/>
        <rdfs:label xml:lang="en">securityArea</rdfs:label>
    </owl:NamedIndividual>
    


    <!-- https://w3id.org/transmodel/facilities#shower -->

    <owl:NamedIndividual rdf:about="https://w3id.org/transmodel/facilities#shower">
        <rdf:type rdf:resource="https://w3id.org/transmodel/facilities#SanitaryEquipment"/>
    </owl:NamedIndividual>
    


    <!-- https://w3id.org/transmodel/facilities#snacks -->

    <owl:NamedIndividual rdf:about="https://w3id.org/transmodel/facilities#snacks"/>
    


    <!-- https://w3id.org/transmodel/facilities#standardBus -->

    <owl:NamedIndividual rdf:about="https://w3id.org/transmodel/facilities#standardBus">
        <rdf:type rdf:resource="https://w3id.org/transmodel/facilities#VehicleType"/>
        <rdfs:label xml:lang="en">standardBus</rdfs:label>
    </owl:NamedIndividual>
    


    <!-- https://w3id.org/transmodel/facilities#stepFree -->

    <owl:NamedIndividual rdf:about="https://w3id.org/transmodel/facilities#stepFree">
        <rdfs:label xml:lang="en">stepFree</rdfs:label>
    </owl:NamedIndividual>
    


    <!-- https://w3id.org/transmodel/facilities#taxRefunds -->

    <owl:NamedIndividual rdf:about="https://w3id.org/transmodel/facilities#taxRefunds"/>
    


    <!-- https://w3id.org/transmodel/facilities#telematicInformationCenter -->

    <owl:NamedIndividual rdf:about="https://w3id.org/transmodel/facilities#telematicInformationCenter">
        <rdfs:comment xml:lang="en">A public transport information piece of Equipment online</rdfs:comment>
        <rdfs:label xml:lang="en">telematicInformationService</rdfs:label>
    </owl:NamedIndividual>
    


    <!-- https://w3id.org/transmodel/facilities#ticketCollection -->

    <owl:NamedIndividual rdf:about="https://w3id.org/transmodel/facilities#ticketCollection"/>
    


    <!-- https://w3id.org/transmodel/facilities#ticketPurchase -->

    <owl:NamedIndividual rdf:about="https://w3id.org/transmodel/facilities#ticketPurchase"/>
    


    <!-- https://w3id.org/transmodel/facilities#toilet -->

    <owl:NamedIndividual rdf:about="https://w3id.org/transmodel/facilities#toilet">
        <rdf:type rdf:resource="https://w3id.org/transmodel/facilities#SanitaryEquipment"/>
    </owl:NamedIndividual>
    


    <!-- https://w3id.org/transmodel/facilities#visualNavigator -->

    <owl:NamedIndividual rdf:about="https://w3id.org/transmodel/facilities#visualNavigator"/>
    


    <!-- https://w3id.org/transmodel/facilities#walkingStick -->

    <owl:NamedIndividual rdf:about="https://w3id.org/transmodel/facilities#walkingStick"/>
    


    <!-- https://w3id.org/transmodel/facilities#weatherConditions -->

    <owl:NamedIndividual rdf:about="https://w3id.org/transmodel/facilities#weatherConditions">
        <rdf:type rdf:resource="https://w3id.org/transmodel/facilities#ValidityTrigger"/>
        <rdfs:label xml:lang="en">weatherConditions</rdfs:label>
    </owl:NamedIndividual>
    


    <!-- https://w3id.org/transmodel/facilities#wheelchair -->

    <owl:NamedIndividual rdf:about="https://w3id.org/transmodel/facilities#wheelchair"/>
    


    <!-- https://w3id.org/transmodel/facilities#wheelchairAccessToilet -->

    <owl:NamedIndividual rdf:about="https://w3id.org/transmodel/facilities#wheelchairAccessToilet">
        <rdf:type rdf:resource="https://w3id.org/transmodel/facilities#SanitaryEquipment"/>
    </owl:NamedIndividual>
    


    <!-- https://w3id.org/transmodel/facilities#wheelchairBabyChange -->

    <owl:NamedIndividual rdf:about="https://w3id.org/transmodel/facilities#wheelchairBabyChange">
        <rdf:type rdf:resource="https://w3id.org/transmodel/facilities#SanitaryEquipment"/>
    </owl:NamedIndividual>
    


    <!-- https://w3id.org/transmodel/kos/facilities/EquipmentType -->

    <owl:NamedIndividual rdf:about="https://w3id.org/transmodel/kos/facilities/EquipmentType">
        <rdf:type rdf:resource="http://www.w3.org/2004/02/skos/core#ConceptScheme"/>
        <rdfs:comment>Concept scheme where all the codelists for the types of equipment that are included in the Transmodel ontology are included</rdfs:comment>
    </owl:NamedIndividual>
    


    <!-- https://w3id.org/transmodel/kos/facilities/FacilityType -->

    <owl:NamedIndividual rdf:about="https://w3id.org/transmodel/kos/facilities/FacilityType">
        <rdf:type rdf:resource="http://www.w3.org/2004/02/skos/core#ConceptScheme"/>
        <rdfs:comment xml:lang="en">Concept scheme where all the codelists for the types of facilities that are included in the Transmodel ontology</rdfs:comment>
    </owl:NamedIndividual>
    


    <!-- https://w3id.org/transmodel/kos/journeys/mobility-limitation -->

    <owl:NamedIndividual rdf:about="https://w3id.org/transmodel/kos/journeys/mobility-limitation">
        <rdfs:comment xml:lang="en">List of concepts regarding Mobility Limitation defined in kos/journeys/mobility-limitation</rdfs:comment>
    </owl:NamedIndividual>

    <rdf:Description>
        <mbox xml:lang="en">adolfo.anton.bravo@upm.es</mbox>
        <name xml:lang="en">Adolfo Anton-Bravo</name>
    </rdf:Description>
    


    <!-- 
    ///////////////////////////////////////////////////////////////////////////////////////
    //
    // General axioms
    //
    ///////////////////////////////////////////////////////////////////////////////////////
     -->

    <rdf:Description>
        <rdf:type rdf:resource="http://www.w3.org/2002/07/owl#AllDisjointClasses"/>
        <owl:members rdf:parseType="Collection">
            <rdf:Description rdf:about="https://w3id.org/transmodel/facilities#HeadingSign"/>
            <rdf:Description rdf:about="https://w3id.org/transmodel/facilities#OtherSign"/>
            <rdf:Description rdf:about="https://w3id.org/transmodel/facilities#PlaceSign"/>
        </owl:members>
    </rdf:Description>
</rdf:RDF>



<!-- Generated by the OWL API (version 4.5.9.2019-02-01T07:24:44Z) https://github.com/owlcs/owlapi -->

